<?xml version="1.0"?>
<rdf:RDF xmlns="https://w3id.org/cop#"
     xml:base="https://w3id.org/cop"
     xmlns:dc="http://purl.org/dc/elements/1.1/"
     xmlns:owl="http://www.w3.org/2002/07/owl#"
     xmlns:rdf="http://www.w3.org/1999/02/22-rdf-syntax-ns#"
     xmlns:xml="http://www.w3.org/XML/1998/namespace"
     xmlns:xsd="http://www.w3.org/2001/XMLSchema#"
     xmlns:bibo="http://purl.org/ontology/bibo/"
     xmlns:doap="http://usefulinc.com/ns/doap#"
     xmlns:foaf="http://xmlns.com/foaf/0.1/"
     xmlns:rdfs="http://www.w3.org/2000/01/rdf-schema#"
     xmlns:skos="http://www.w3.org/2004/02/skos/core#"
     xmlns:vann="http://purl.org/vocab/vann/"
     xmlns:terms="http://purl.org/dc/terms/">
    <owl:Ontology rdf:about="https://w3id.org/cop">
        <owl:versionIRI rdf:resource="https://w3id.org/cop/release/2025-03-18"/>
        <owl:imports rdf:resource="https://w3id.org/gfo-light/release/2025-03-17"/>
        <dc:created rdf:datatype="http://www.w3.org/2001/XMLSchema#date">2020-01-20</dc:created>
        <dc:creator>Alexandr Uciteli</dc:creator>
        <dc:creator>Christoph Beger</dc:creator>
        <dc:creator>Franz Matthies</dc:creator>
        <dc:creator>Konrad Höffner</dc:creator>
        <dc:creator>Ralph Schäfermeier</dc:creator>
        <dc:description xml:lang="de">Die Core Ontology of Phenotyping (COP) definiert zentrale Entitäten und ihre Beziehungen, die für die Modellierung phänotypischen Wissens und die Entwicklung von Software für die Phänotypisierung relevant sind.</dc:description>
        <dc:description xml:lang="en">The Core Ontology of Phenotyping (COP) defines core entities and their relationships that are relevant for modelling phenotypic knowledge and developing phenotyping software.</dc:description>
        <dc:modified rdf:datatype="http://www.w3.org/2001/XMLSchema#date">2025-03-18</dc:modified>
        <dc:title xml:lang="en">Core Ontology of Phenotyping (COP)</dc:title>
        <terms:license rdf:resource="http://creativecommons.org/licenses/by/4.0/"/>
        <bibo:doi rdf:resource="https://zenodo.org/doi/10.5281/zenodo.5205497"/>
        <vann:preferredNamespacePrefix>cop</vann:preferredNamespacePrefix>
        <vann:preferredNamespaceURI>https://w3id.org/cop/</vann:preferredNamespaceURI>
        <doap:repository rdf:resource="https://github.com/Onto-Med/COP"/>
        <rdfs:label xml:lang="en">Core Ontology of Phenotyping</rdfs:label>
        <owl:priorVersion rdf:resource="https://w3id.org/cop/release/2024-07-08"/>
        <owl:versionInfo rdf:datatype="http://www.w3.org/2001/XMLSchema#date">2025-03-18</owl:versionInfo>
        <foaf:homepage rdf:resource="https://github.com/Onto-Med/COP"/>
    </owl:Ontology>
    


    <!-- 
    ///////////////////////////////////////////////////////////////////////////////////////
    //
    // Annotation properties
    //
    ///////////////////////////////////////////////////////////////////////////////////////
     -->


    


    <!-- http://purl.org/dc/elements/1.1/contributor -->


    <owl:AnnotationProperty rdf:about="http://purl.org/dc/elements/1.1/contributor"/>
    


    <!-- http://purl.org/dc/elements/1.1/created -->


    <owl:AnnotationProperty rdf:about="http://purl.org/dc/elements/1.1/created"/>
    


    <!-- http://purl.org/dc/elements/1.1/creator -->


    <owl:AnnotationProperty rdf:about="http://purl.org/dc/elements/1.1/creator"/>
    


    <!-- http://purl.org/dc/elements/1.1/description -->


    <owl:AnnotationProperty rdf:about="http://purl.org/dc/elements/1.1/description"/>
    


    <!-- http://purl.org/dc/elements/1.1/modified -->


    <owl:AnnotationProperty rdf:about="http://purl.org/dc/elements/1.1/modified"/>
    


    <!-- http://purl.org/dc/elements/1.1/title -->


    <owl:AnnotationProperty rdf:about="http://purl.org/dc/elements/1.1/title"/>
    


    <!-- http://purl.org/dc/terms/license -->


    <owl:AnnotationProperty rdf:about="http://purl.org/dc/terms/license"/>
    


    <!-- http://purl.org/dc/terms/references -->


    <owl:AnnotationProperty rdf:about="http://purl.org/dc/terms/references"/>
    


    <!-- http://purl.org/ontology/bibo/doi -->


    <owl:AnnotationProperty rdf:about="http://purl.org/ontology/bibo/doi"/>
    


    <!-- http://purl.org/vocab/vann/preferredNamespacePrefix -->


    <owl:AnnotationProperty rdf:about="http://purl.org/vocab/vann/preferredNamespacePrefix"/>
    


    <!-- http://purl.org/vocab/vann/preferredNamespaceURI -->


    <owl:AnnotationProperty rdf:about="http://purl.org/vocab/vann/preferredNamespaceURI"/>
    


    <!-- http://usefulinc.com/ns/doap#repository -->


    <owl:AnnotationProperty rdf:about="http://usefulinc.com/ns/doap#repository"/>
    


    <!-- http://www.w3.org/2000/01/rdf-schema#comment -->


    <owl:AnnotationProperty rdf:about="http://www.w3.org/2000/01/rdf-schema#comment"/>
    


    <!-- http://www.w3.org/2002/07/owl#versionInfo -->


    <owl:AnnotationProperty rdf:about="http://www.w3.org/2002/07/owl#versionInfo"/>
    


    <!-- http://www.w3.org/2004/02/skos/core#altLabel -->


    <owl:AnnotationProperty rdf:about="http://www.w3.org/2004/02/skos/core#altLabel"/>
    


    <!-- http://www.w3.org/2004/02/skos/core#definition -->


    <owl:AnnotationProperty rdf:about="http://www.w3.org/2004/02/skos/core#definition"/>
    


    <!-- http://www.w3.org/2004/02/skos/core#example -->


    <owl:AnnotationProperty rdf:about="http://www.w3.org/2004/02/skos/core#example"/>
    


    <!-- http://xmlns.com/foaf/0.1/homepage -->


    <owl:AnnotationProperty rdf:about="http://xmlns.com/foaf/0.1/homepage"/>
    


    <!-- 
    ///////////////////////////////////////////////////////////////////////////////////////
    //
    // Datatypes
    //
    ///////////////////////////////////////////////////////////////////////////////////////
     -->


    


    <!-- http://www.w3.org/2001/XMLSchema#date -->


    <rdfs:Datatype rdf:about="http://www.w3.org/2001/XMLSchema#date"/>
    


    <!-- 
    ///////////////////////////////////////////////////////////////////////////////////////
    //
    // Object Properties
    //
    ///////////////////////////////////////////////////////////////////////////////////////
     -->


    


    <!-- https://w3id.org/cop/applicableFor -->


    <owl:ObjectProperty rdf:about="https://w3id.org/cop/applicableFor">
        <rdfs:domain rdf:resource="https://w3id.org/cop/PhenotypeAlgorithm"/>
        <rdfs:range rdf:resource="https://w3id.org/cop/PhenotypeQuery"/>
        <rdfs:label xml:lang="en">applicable for</rdfs:label>
    </owl:ObjectProperty>
    


    <!-- https://w3id.org/cop/basedOn -->


    <owl:ObjectProperty rdf:about="https://w3id.org/cop/basedOn">
        <rdfs:domain rdf:resource="https://w3id.org/cop/PhenotypeQuery"/>
        <rdfs:range rdf:resource="https://w3id.org/cop/PhenotypeModel"/>
        <rdfs:label xml:lang="en">based on</rdfs:label>
    </owl:ObjectProperty>
    


    <!-- https://w3id.org/cop/basicRestrictionOf -->


    <owl:ObjectProperty rdf:about="https://w3id.org/cop/basicRestrictionOf">
        <rdfs:domain rdf:resource="https://w3id.org/cop/BasicRestrictedPhenotypeClassView"/>
        <rdfs:range rdf:resource="https://w3id.org/cop/BasicUnrestrictedPhenotypeClassView"/>
        <rdfs:label xml:lang="en">basic restriction of</rdfs:label>
    </owl:ObjectProperty>
    


    <!-- https://w3id.org/cop/derivedFrom -->


    <owl:ObjectProperty rdf:about="https://w3id.org/cop/derivedFrom">
        <rdfs:domain rdf:resource="https://w3id.org/cop/DerivedUnrestrictedPhenotypeClassView"/>
        <rdfs:range rdf:resource="https://w3id.org/cop/PhenotypeClassView"/>
        <rdfs:label xml:lang="en">derived from</rdfs:label>
    </owl:ObjectProperty>
    


    <!-- https://w3id.org/cop/derivedRestrictionOf -->


    <owl:ObjectProperty rdf:about="https://w3id.org/cop/derivedRestrictionOf">
        <rdfs:domain rdf:resource="https://w3id.org/cop/DerivedRestrictedPhenotypeClassView"/>
        <rdfs:range rdf:resource="https://w3id.org/cop/DerivedUnrestrictedPhenotypeClassView"/>
        <rdfs:label xml:lang="en">derived restriction of</rdfs:label>
    </owl:ObjectProperty>
    


    <!-- https://w3id.org/cop/hasExclusion -->


    <owl:ObjectProperty rdf:about="https://w3id.org/cop/hasExclusion">
        <rdfs:subPropertyOf rdf:resource="https://w3id.org/cop/hasQueryParameter"/>
        <rdfs:label xml:lang="en">has exclusion</rdfs:label>
    </owl:ObjectProperty>
    


    <!-- https://w3id.org/cop/hasInclusion -->


    <owl:ObjectProperty rdf:about="https://w3id.org/cop/hasInclusion">
        <rdfs:subPropertyOf rdf:resource="https://w3id.org/cop/hasQueryParameter"/>
        <rdfs:label xml:lang="en">has inclusion</rdfs:label>
    </owl:ObjectProperty>
    


    <!-- https://w3id.org/cop/hasProjection -->


    <owl:ObjectProperty rdf:about="https://w3id.org/cop/hasProjection">
        <rdfs:subPropertyOf rdf:resource="https://w3id.org/cop/hasQueryParameter"/>
        <rdfs:label xml:lang="en">has projection</rdfs:label>
    </owl:ObjectProperty>
    


    <!-- https://w3id.org/cop/hasQueryParameter -->


    <owl:ObjectProperty rdf:about="https://w3id.org/cop/hasQueryParameter">
        <rdfs:subPropertyOf rdf:resource="https://w3id.org/gfo-light/hasPart"/>
        <rdfs:domain rdf:resource="https://w3id.org/cop/PhenotypeQuery"/>
        <rdfs:range rdf:resource="https://w3id.org/cop/PhenotypeClassView"/>
        <rdfs:label xml:lang="en">has query parameter</rdfs:label>
    </owl:ObjectProperty>
    


    <!-- https://w3id.org/cop/hasVariable -->


    <owl:ObjectProperty rdf:about="https://w3id.org/cop/hasVariable">
        <rdfs:subPropertyOf rdf:resource="https://w3id.org/gfo-light/hasPart"/>
        <rdfs:domain rdf:resource="https://w3id.org/cop/DerivationExpression"/>
        <rdfs:range rdf:resource="https://w3id.org/cop/PhenotypeClassView"/>
        <rdfs:label xml:lang="en">has variable</rdfs:label>
    </owl:ObjectProperty>
    


    <!-- https://w3id.org/cop/identifies -->


    <owl:ObjectProperty rdf:about="https://w3id.org/cop/identifies">
        <rdfs:domain rdf:resource="https://w3id.org/cop/Phenotyping"/>
        <rdfs:range rdf:resource="https://w3id.org/cop/Organism"/>
        <rdfs:label xml:lang="en">identifies</rdfs:label>
    </owl:ObjectProperty>
    


    <!-- https://w3id.org/cop/implementedBy -->


    <owl:ObjectProperty rdf:about="https://w3id.org/cop/implementedBy">
        <owl:inverseOf rdf:resource="https://w3id.org/cop/implements"/>
        <rdfs:domain rdf:resource="https://w3id.org/cop/Algorithm"/>
        <rdfs:range rdf:resource="https://w3id.org/cop/Software"/>
        <rdfs:label xml:lang="en">implemented by</rdfs:label>
    </owl:ObjectProperty>
    


    <!-- https://w3id.org/cop/implements -->


    <owl:ObjectProperty rdf:about="https://w3id.org/cop/implements">
        <rdfs:domain rdf:resource="https://w3id.org/cop/Software"/>
        <rdfs:range rdf:resource="https://w3id.org/cop/Algorithm"/>
        <rdfs:label xml:lang="en">implements</rdfs:label>
    </owl:ObjectProperty>
    


    <!-- https://w3id.org/cop/realises -->


    <owl:ObjectProperty rdf:about="https://w3id.org/cop/realises">
        <rdfs:domain rdf:resource="https://w3id.org/cop/Software"/>
        <rdfs:range rdf:resource="https://w3id.org/gfo-light/Process"/>
        <rdfs:label xml:lang="en">realises</rdfs:label>
    </owl:ObjectProperty>
    


    <!-- https://w3id.org/cop/restrictionOf -->


    <owl:ObjectProperty rdf:about="https://w3id.org/cop/restrictionOf">
        <rdfs:domain rdf:resource="https://w3id.org/cop/RestrictedPhenotypeClass"/>
        <rdfs:range rdf:resource="https://w3id.org/cop/UnrestrictedPhenotypeClass"/>
        <rdfs:label xml:lang="en">restriction of</rdfs:label>
    </owl:ObjectProperty>
    


    <!-- https://w3id.org/gfo-light/after -->


    <owl:ObjectProperty rdf:about="https://w3id.org/gfo-light/after">
        <rdfs:subPropertyOf rdf:resource="https://w3id.org/gfo-light/temporallyRelatedWith"/>
        <owl:inverseOf rdf:resource="https://w3id.org/gfo-light/before"/>
        <rdfs:label xml:lang="en">after</rdfs:label>
    </owl:ObjectProperty>
    


    <!-- https://w3id.org/gfo-light/attributiveOf -->


    <owl:ObjectProperty rdf:about="https://w3id.org/gfo-light/attributiveOf">
        <owl:inverseOf rdf:resource="https://w3id.org/gfo-light/hasAttributive"/>
        <rdfs:domain rdf:resource="https://w3id.org/gfo-light/Attributive"/>
        <rdfs:range rdf:resource="https://w3id.org/gfo-light/Individual"/>
        <rdfs:label xml:lang="en">attributive of</rdfs:label>
    </owl:ObjectProperty>
    


    <!-- https://w3id.org/gfo-light/before -->


    <owl:ObjectProperty rdf:about="https://w3id.org/gfo-light/before">
        <rdfs:subPropertyOf rdf:resource="https://w3id.org/gfo-light/temporallyRelatedWith"/>
        <rdfs:label xml:lang="en">before</rdfs:label>
        <skos:definition xml:lang="en">X before Y: Xf &lt; Ys</skos:definition>
    </owl:ObjectProperty>
    


    <!-- https://w3id.org/gfo-light/boundaryOf -->


    <owl:ObjectProperty rdf:about="https://w3id.org/gfo-light/boundaryOf">
        <owl:inverseOf rdf:resource="https://w3id.org/gfo-light/hasBoundary"/>
        <rdfs:domain rdf:resource="https://w3id.org/gfo-light/ObjectBoundary"/>
        <rdfs:range>
            <owl:Class>
                <owl:unionOf rdf:parseType="Collection">
                    <rdf:Description rdf:about="https://w3id.org/gfo-light/Line"/>
                    <rdf:Description rdf:about="https://w3id.org/gfo-light/Object"/>
                    <rdf:Description rdf:about="https://w3id.org/gfo-light/Surface"/>
                </owl:unionOf>
            </owl:Class>
        </rdfs:range>
        <rdfs:label xml:lang="en">boundary of</rdfs:label>
    </owl:ObjectProperty>
    


    <!-- https://w3id.org/gfo-light/causedBy -->


    <owl:ObjectProperty rdf:about="https://w3id.org/gfo-light/causedBy">
        <rdfs:subPropertyOf rdf:resource="https://w3id.org/gfo-light/resultsFrom"/>
        <owl:inverseOf rdf:resource="https://w3id.org/gfo-light/causes"/>
        <rdfs:label xml:lang="en">caused by</rdfs:label>
    </owl:ObjectProperty>
    


    <!-- https://w3id.org/gfo-light/causes -->


    <owl:ObjectProperty rdf:about="https://w3id.org/gfo-light/causes">
        <rdfs:subPropertyOf rdf:resource="https://w3id.org/gfo-light/leadsTo"/>
        <rdfs:label xml:lang="en">causes</rdfs:label>
    </owl:ObjectProperty>
    


    <!-- https://w3id.org/gfo-light/containsRole -->


    <owl:ObjectProperty rdf:about="https://w3id.org/gfo-light/containsRole">
        <owl:inverseOf rdf:resource="https://w3id.org/gfo-light/roleIn"/>
        <rdfs:domain>
            <owl:Class>
                <owl:unionOf rdf:parseType="Collection">
                    <rdf:Description rdf:about="https://w3id.org/gfo-light/Object"/>
                    <rdf:Description rdf:about="https://w3id.org/gfo-light/ObjectAggregate"/>
                    <rdf:Description rdf:about="https://w3id.org/gfo-light/ProcessualEntity"/>
                    <rdf:Description rdf:about="https://w3id.org/gfo-light/Relator"/>
                    <rdf:Description rdf:about="https://w3id.org/gfo-light/SituationalEntity"/>
                </owl:unionOf>
            </owl:Class>
        </rdfs:domain>
        <rdfs:range rdf:resource="https://w3id.org/gfo-light/Role"/>
        <rdfs:label xml:lang="en">contains role</rdfs:label>
    </owl:ObjectProperty>
    


    <!-- https://w3id.org/gfo-light/during -->


    <owl:ObjectProperty rdf:about="https://w3id.org/gfo-light/during">
        <rdfs:subPropertyOf rdf:resource="https://w3id.org/gfo-light/temporalPartOf"/>
        <owl:inverseOf rdf:resource="https://w3id.org/gfo-light/temporallyContains"/>
        <rdfs:label xml:lang="en">during</rdfs:label>
        <skos:definition xml:lang="en">X during Y: Xs &gt; Ys and Xf &lt; Yf</skos:definition>
    </owl:ObjectProperty>
    


    <!-- https://w3id.org/gfo-light/hasAttributive -->


    <owl:ObjectProperty rdf:about="https://w3id.org/gfo-light/hasAttributive">
        <rdfs:domain rdf:resource="https://w3id.org/gfo-light/Individual"/>
        <rdfs:range rdf:resource="https://w3id.org/gfo-light/Attributive"/>
        <rdfs:label xml:lang="en">has attributive</rdfs:label>
    </owl:ObjectProperty>
    


    <!-- https://w3id.org/gfo-light/hasBoundary -->


    <owl:ObjectProperty rdf:about="https://w3id.org/gfo-light/hasBoundary">
        <rdfs:domain>
            <owl:Class>
                <owl:unionOf rdf:parseType="Collection">
                    <rdf:Description rdf:about="https://w3id.org/gfo-light/Line"/>
                    <rdf:Description rdf:about="https://w3id.org/gfo-light/Object"/>
                    <rdf:Description rdf:about="https://w3id.org/gfo-light/Surface"/>
                </owl:unionOf>
            </owl:Class>
        </rdfs:domain>
        <rdfs:range rdf:resource="https://w3id.org/gfo-light/ObjectBoundary"/>
        <rdfs:label xml:lang="en">has boundary</rdfs:label>
    </owl:ObjectProperty>
    


    <!-- https://w3id.org/gfo-light/hasInnerBoundary -->


    <owl:ObjectProperty rdf:about="https://w3id.org/gfo-light/hasInnerBoundary">
        <rdfs:subPropertyOf rdf:resource="https://w3id.org/gfo-light/hasBoundary"/>
        <owl:inverseOf rdf:resource="https://w3id.org/gfo-light/innerBoundaryOf"/>
        <rdfs:label xml:lang="en">has inner boundary</rdfs:label>
    </owl:ObjectProperty>
    


    <!-- https://w3id.org/gfo-light/hasMember -->


    <owl:ObjectProperty rdf:about="https://w3id.org/gfo-light/hasMember">
        <owl:inverseOf rdf:resource="https://w3id.org/gfo-light/memberOf"/>
        <rdfs:domain>
            <owl:Class>
                <owl:unionOf rdf:parseType="Collection">
                    <rdf:Description rdf:about="https://w3id.org/gfo-light/ObjectAggregate"/>
                    <rdf:Description rdf:about="https://w3id.org/gfo-light/ProcessAggregate"/>
                    <rdf:Description rdf:about="https://w3id.org/gfo-light/SituationAggregate"/>
                </owl:unionOf>
            </owl:Class>
        </rdfs:domain>
        <rdfs:range>
            <owl:Class>
                <owl:unionOf rdf:parseType="Collection">
                    <rdf:Description rdf:about="https://w3id.org/gfo-light/Object"/>
                    <rdf:Description rdf:about="https://w3id.org/gfo-light/ObjectAggregate"/>
                    <rdf:Description rdf:about="https://w3id.org/gfo-light/ProcessualEntity"/>
                    <rdf:Description rdf:about="https://w3id.org/gfo-light/SituationalEntity"/>
                </owl:unionOf>
            </owl:Class>
        </rdfs:range>
        <rdfs:label xml:lang="en">has member</rdfs:label>
    </owl:ObjectProperty>
    


    <!-- https://w3id.org/gfo-light/hasNaturalBoundary -->


    <owl:ObjectProperty rdf:about="https://w3id.org/gfo-light/hasNaturalBoundary">
        <rdfs:subPropertyOf rdf:resource="https://w3id.org/gfo-light/hasBoundary"/>
        <owl:inverseOf rdf:resource="https://w3id.org/gfo-light/naturalBoundaryOf"/>
        <rdfs:label xml:lang="en">has natural boundary</rdfs:label>
    </owl:ObjectProperty>
    


    <!-- https://w3id.org/gfo-light/hasOwner -->


    <owl:ObjectProperty rdf:about="https://w3id.org/gfo-light/hasOwner">
        <owl:inverseOf rdf:resource="https://w3id.org/gfo-light/ownerOf"/>
        <rdfs:domain rdf:resource="https://w3id.org/gfo-light/ObjectBoundary"/>
        <rdfs:range rdf:resource="https://w3id.org/gfo-light/Object"/>
        <rdfs:label xml:lang="en">has owner</rdfs:label>
    </owl:ObjectProperty>
    


    <!-- https://w3id.org/gfo-light/hasPart -->


    <owl:ObjectProperty rdf:about="https://w3id.org/gfo-light/hasPart">
        <owl:inverseOf rdf:resource="https://w3id.org/gfo-light/partOf"/>
        <rdfs:domain rdf:resource="https://w3id.org/gfo-light/Individual"/>
        <rdfs:range rdf:resource="https://w3id.org/gfo-light/Individual"/>
        <rdfs:label xml:lang="en">has part</rdfs:label>
    </owl:ObjectProperty>
    


    <!-- https://w3id.org/gfo-light/hasParticipant -->


    <owl:ObjectProperty rdf:about="https://w3id.org/gfo-light/hasParticipant">
        <owl:inverseOf rdf:resource="https://w3id.org/gfo-light/participatesIn"/>
        <rdfs:domain>
            <owl:Class>
                <owl:unionOf rdf:parseType="Collection">
                    <rdf:Description rdf:about="https://w3id.org/gfo-light/ProcessualEntity"/>
                    <rdf:Description rdf:about="https://w3id.org/gfo-light/SituationalEntity"/>
                </owl:unionOf>
            </owl:Class>
        </rdfs:domain>
        <rdfs:range rdf:resource="https://w3id.org/gfo-light/Continuant"/>
        <rdfs:label xml:lang="en">has participant</rdfs:label>
    </owl:ObjectProperty>
    


    <!-- https://w3id.org/gfo-light/hasProcessPart -->


    <owl:ObjectProperty rdf:about="https://w3id.org/gfo-light/hasProcessPart">
        <rdfs:subPropertyOf rdf:resource="https://w3id.org/gfo-light/hasPart"/>
        <owl:inverseOf rdf:resource="https://w3id.org/gfo-light/processPartOf"/>
        <rdfs:domain rdf:resource="https://w3id.org/gfo-light/Process"/>
        <rdfs:range>
            <owl:Class>
                <owl:unionOf rdf:parseType="Collection">
                    <rdf:Description rdf:about="https://w3id.org/gfo-light/Attributive"/>
                    <rdf:Description rdf:about="https://w3id.org/gfo-light/Process"/>
                    <rdf:Description rdf:about="https://w3id.org/gfo-light/Situation"/>
                </owl:unionOf>
            </owl:Class>
        </rdfs:range>
        <rdfs:label xml:lang="en">has process part</rdfs:label>
    </owl:ObjectProperty>
    


    <!-- https://w3id.org/gfo-light/hasQuality -->


    <owl:ObjectProperty rdf:about="https://w3id.org/gfo-light/hasQuality">
        <rdfs:subPropertyOf rdf:resource="https://w3id.org/gfo-light/hasAttributive"/>
        <owl:inverseOf rdf:resource="https://w3id.org/gfo-light/qualityOf"/>
        <rdfs:domain rdf:resource="https://w3id.org/gfo-light/Individual"/>
        <rdfs:range rdf:resource="https://w3id.org/gfo-light/Quality"/>
        <rdfs:label xml:lang="en">has quality</rdfs:label>
    </owl:ObjectProperty>
    


    <!-- https://w3id.org/gfo-light/hasSituationPart -->


    <owl:ObjectProperty rdf:about="https://w3id.org/gfo-light/hasSituationPart">
        <rdfs:subPropertyOf rdf:resource="https://w3id.org/gfo-light/hasPart"/>
        <owl:inverseOf rdf:resource="https://w3id.org/gfo-light/situationPartOf"/>
        <rdfs:domain rdf:resource="https://w3id.org/gfo-light/Situation"/>
        <rdfs:range>
            <owl:Class>
                <owl:unionOf rdf:parseType="Collection">
                    <rdf:Description rdf:about="https://w3id.org/gfo-light/Attributive"/>
                    <rdf:Description rdf:about="https://w3id.org/gfo-light/Situation"/>
                </owl:unionOf>
            </owl:Class>
        </rdfs:range>
        <rdfs:label xml:lang="en">has situation part</rdfs:label>
    </owl:ObjectProperty>
    


    <!-- https://w3id.org/gfo-light/hasTemporalPart -->


    <owl:ObjectProperty rdf:about="https://w3id.org/gfo-light/hasTemporalPart">
        <rdfs:subPropertyOf rdf:resource="https://w3id.org/gfo-light/temporallyRelatedWith"/>
        <owl:inverseOf rdf:resource="https://w3id.org/gfo-light/temporalPartOf"/>
        <rdfs:label xml:lang="en">has temporal part</rdfs:label>
    </owl:ObjectProperty>
    


    <!-- https://w3id.org/gfo-light/hasTime -->


    <owl:ObjectProperty rdf:about="https://w3id.org/gfo-light/hasTime">
        <owl:inverseOf rdf:resource="https://w3id.org/gfo-light/timeOf"/>
        <rdfs:domain rdf:resource="https://w3id.org/gfo-light/ConcreteIndividual"/>
        <rdfs:range rdf:resource="https://w3id.org/gfo-light/TimeEntity"/>
        <rdfs:label xml:lang="en">has time</rdfs:label>
    </owl:ObjectProperty>
    


    <!-- https://w3id.org/gfo-light/innerBoundaryOf -->


    <owl:ObjectProperty rdf:about="https://w3id.org/gfo-light/innerBoundaryOf">
        <rdfs:subPropertyOf rdf:resource="https://w3id.org/gfo-light/boundaryOf"/>
        <rdfs:label xml:lang="en">inner boundary of</rdfs:label>
    </owl:ObjectProperty>
    


    <!-- https://w3id.org/gfo-light/instanceOf -->


    <owl:ObjectProperty rdf:about="https://w3id.org/gfo-light/instanceOf">
        <owl:inverseOf rdf:resource="https://w3id.org/gfo-light/instantiatedBy"/>
        <rdfs:domain rdf:resource="https://w3id.org/gfo-light/Entity"/>
        <rdfs:range rdf:resource="https://w3id.org/gfo-light/Category"/>
        <rdfs:label xml:lang="en">instance of</rdfs:label>
    </owl:ObjectProperty>
    


    <!-- https://w3id.org/gfo-light/instantiatedBy -->


    <owl:ObjectProperty rdf:about="https://w3id.org/gfo-light/instantiatedBy">
        <rdfs:domain rdf:resource="https://w3id.org/gfo-light/Category"/>
        <rdfs:range rdf:resource="https://w3id.org/gfo-light/Entity"/>
        <rdfs:label xml:lang="en">instantiated by</rdfs:label>
    </owl:ObjectProperty>
    


    <!-- https://w3id.org/gfo-light/leadsTo -->


    <owl:ObjectProperty rdf:about="https://w3id.org/gfo-light/leadsTo">
        <owl:inverseOf rdf:resource="https://w3id.org/gfo-light/resultsFrom"/>
        <rdfs:domain>
            <owl:Class>
                <owl:unionOf rdf:parseType="Collection">
                    <rdf:Description rdf:about="https://w3id.org/gfo-light/ProcessualEntity"/>
                    <rdf:Description rdf:about="https://w3id.org/gfo-light/SituationalEntity"/>
                </owl:unionOf>
            </owl:Class>
        </rdfs:domain>
        <rdfs:range>
            <owl:Class>
                <owl:unionOf rdf:parseType="Collection">
                    <rdf:Description rdf:about="https://w3id.org/gfo-light/ProcessualEntity"/>
                    <rdf:Description rdf:about="https://w3id.org/gfo-light/SituationalEntity"/>
                </owl:unionOf>
            </owl:Class>
        </rdfs:range>
        <rdfs:label xml:lang="en">leads to</rdfs:label>
    </owl:ObjectProperty>
    


    <!-- https://w3id.org/gfo-light/locatedIn -->


    <owl:ObjectProperty rdf:about="https://w3id.org/gfo-light/locatedIn">
        <owl:inverseOf rdf:resource="https://w3id.org/gfo-light/locationOf"/>
        <rdfs:domain>
            <owl:Class>
                <owl:unionOf rdf:parseType="Collection">
                    <rdf:Description rdf:about="https://w3id.org/gfo-light/Object"/>
                    <rdf:Description rdf:about="https://w3id.org/gfo-light/ProcessualEntity"/>
                    <rdf:Description rdf:about="https://w3id.org/gfo-light/SituationalEntity"/>
                </owl:unionOf>
            </owl:Class>
        </rdfs:domain>
        <rdfs:range rdf:resource="https://w3id.org/gfo-light/Object"/>
        <rdfs:comment xml:lang="en">Material objects can be located in other material objects (locatedIn, e.g., the driver is located in the car).</rdfs:comment>
        <rdfs:comment xml:lang="en">Processes and situations can take place (locatedIn) in material objects (e.g., a football match in a stadium or an illness in a person).</rdfs:comment>
        <rdfs:label xml:lang="en">located in</rdfs:label>
    </owl:ObjectProperty>
    


    <!-- https://w3id.org/gfo-light/locationOf -->


    <owl:ObjectProperty rdf:about="https://w3id.org/gfo-light/locationOf">
        <rdfs:domain rdf:resource="https://w3id.org/gfo-light/Object"/>
        <rdfs:range>
            <owl:Class>
                <owl:unionOf rdf:parseType="Collection">
                    <rdf:Description rdf:about="https://w3id.org/gfo-light/Object"/>
                    <rdf:Description rdf:about="https://w3id.org/gfo-light/ProcessualEntity"/>
                    <rdf:Description rdf:about="https://w3id.org/gfo-light/SituationalEntity"/>
                </owl:unionOf>
            </owl:Class>
        </rdfs:range>
        <rdfs:label xml:lang="en">location of</rdfs:label>
    </owl:ObjectProperty>
    


    <!-- https://w3id.org/gfo-light/memberOf -->


    <owl:ObjectProperty rdf:about="https://w3id.org/gfo-light/memberOf">
        <rdfs:domain>
            <owl:Class>
                <owl:unionOf rdf:parseType="Collection">
                    <rdf:Description rdf:about="https://w3id.org/gfo-light/Object"/>
                    <rdf:Description rdf:about="https://w3id.org/gfo-light/ObjectAggregate"/>
                    <rdf:Description rdf:about="https://w3id.org/gfo-light/ProcessualEntity"/>
                    <rdf:Description rdf:about="https://w3id.org/gfo-light/SituationalEntity"/>
                </owl:unionOf>
            </owl:Class>
        </rdfs:domain>
        <rdfs:range>
            <owl:Class>
                <owl:unionOf rdf:parseType="Collection">
                    <rdf:Description rdf:about="https://w3id.org/gfo-light/ObjectAggregate"/>
                    <rdf:Description rdf:about="https://w3id.org/gfo-light/ProcessAggregate"/>
                    <rdf:Description rdf:about="https://w3id.org/gfo-light/SituationAggregate"/>
                </owl:unionOf>
            </owl:Class>
        </rdfs:range>
        <rdfs:label xml:lang="en">member of</rdfs:label>
    </owl:ObjectProperty>
    


    <!-- https://w3id.org/gfo-light/naturalBoundaryOf -->


    <owl:ObjectProperty rdf:about="https://w3id.org/gfo-light/naturalBoundaryOf">
        <rdfs:subPropertyOf rdf:resource="https://w3id.org/gfo-light/boundaryOf"/>
        <rdfs:label xml:lang="en">natural boundary of</rdfs:label>
    </owl:ObjectProperty>
    


    <!-- https://w3id.org/gfo-light/ownerOf -->


    <owl:ObjectProperty rdf:about="https://w3id.org/gfo-light/ownerOf">
        <rdfs:domain rdf:resource="https://w3id.org/gfo-light/Object"/>
        <rdfs:range rdf:resource="https://w3id.org/gfo-light/ObjectBoundary"/>
        <rdfs:label xml:lang="en">owner of</rdfs:label>
    </owl:ObjectProperty>
    


    <!-- https://w3id.org/gfo-light/partOf -->


    <owl:ObjectProperty rdf:about="https://w3id.org/gfo-light/partOf">
        <rdfs:domain rdf:resource="https://w3id.org/gfo-light/Individual"/>
        <rdfs:range rdf:resource="https://w3id.org/gfo-light/Individual"/>
        <rdfs:label xml:lang="en">part of</rdfs:label>
    </owl:ObjectProperty>
    


    <!-- https://w3id.org/gfo-light/participatesIn -->


    <owl:ObjectProperty rdf:about="https://w3id.org/gfo-light/participatesIn">
        <rdfs:domain rdf:resource="https://w3id.org/gfo-light/Continuant"/>
        <rdfs:range>
            <owl:Class>
                <owl:unionOf rdf:parseType="Collection">
                    <rdf:Description rdf:about="https://w3id.org/gfo-light/ProcessualEntity"/>
                    <rdf:Description rdf:about="https://w3id.org/gfo-light/SituationalEntity"/>
                </owl:unionOf>
            </owl:Class>
        </rdfs:range>
        <rdfs:label xml:lang="en">participates in</rdfs:label>
    </owl:ObjectProperty>
    


    <!-- https://w3id.org/gfo-light/playedBy -->


    <owl:ObjectProperty rdf:about="https://w3id.org/gfo-light/playedBy">
        <rdfs:subPropertyOf rdf:resource="https://w3id.org/gfo-light/attributiveOf"/>
        <owl:inverseOf rdf:resource="https://w3id.org/gfo-light/plays"/>
        <rdfs:domain rdf:resource="https://w3id.org/gfo-light/Role"/>
        <rdfs:range rdf:resource="https://w3id.org/gfo-light/Continuant"/>
        <rdfs:label xml:lang="en">played by</rdfs:label>
    </owl:ObjectProperty>
    


    <!-- https://w3id.org/gfo-light/plays -->


    <owl:ObjectProperty rdf:about="https://w3id.org/gfo-light/plays">
        <rdfs:subPropertyOf rdf:resource="https://w3id.org/gfo-light/hasAttributive"/>
        <rdfs:domain rdf:resource="https://w3id.org/gfo-light/Continuant"/>
        <rdfs:range rdf:resource="https://w3id.org/gfo-light/Role"/>
        <rdfs:label xml:lang="en">plays</rdfs:label>
    </owl:ObjectProperty>
    


    <!-- https://w3id.org/gfo-light/processPartOf -->


    <owl:ObjectProperty rdf:about="https://w3id.org/gfo-light/processPartOf">
        <rdfs:subPropertyOf rdf:resource="https://w3id.org/gfo-light/partOf"/>
        <rdfs:domain>
            <owl:Class>
                <owl:unionOf rdf:parseType="Collection">
                    <rdf:Description rdf:about="https://w3id.org/gfo-light/Attributive"/>
                    <rdf:Description rdf:about="https://w3id.org/gfo-light/Process"/>
                    <rdf:Description rdf:about="https://w3id.org/gfo-light/Situation"/>
                </owl:unionOf>
            </owl:Class>
        </rdfs:domain>
        <rdfs:range rdf:resource="https://w3id.org/gfo-light/Process"/>
        <rdfs:label xml:lang="en">process part of</rdfs:label>
    </owl:ObjectProperty>
    


    <!-- https://w3id.org/gfo-light/qualityOf -->


    <owl:ObjectProperty rdf:about="https://w3id.org/gfo-light/qualityOf">
        <rdfs:subPropertyOf rdf:resource="https://w3id.org/gfo-light/attributiveOf"/>
        <rdfs:domain rdf:resource="https://w3id.org/gfo-light/Quality"/>
        <rdfs:range rdf:resource="https://w3id.org/gfo-light/Individual"/>
        <rdfs:label xml:lang="en">quality of</rdfs:label>
    </owl:ObjectProperty>
    


    <!-- https://w3id.org/gfo-light/relatedBy -->


    <owl:ObjectProperty rdf:about="https://w3id.org/gfo-light/relatedBy">
        <rdfs:subPropertyOf rdf:resource="https://w3id.org/gfo-light/hasAttributive"/>
        <owl:inverseOf rdf:resource="https://w3id.org/gfo-light/relates"/>
        <rdfs:domain rdf:resource="https://w3id.org/gfo-light/Continuant"/>
        <rdfs:range rdf:resource="https://w3id.org/gfo-light/Relator"/>
        <rdfs:label xml:lang="en">related by</rdfs:label>
    </owl:ObjectProperty>
    


    <!-- https://w3id.org/gfo-light/relates -->


    <owl:ObjectProperty rdf:about="https://w3id.org/gfo-light/relates">
        <rdfs:subPropertyOf rdf:resource="https://w3id.org/gfo-light/attributiveOf"/>
        <rdfs:domain rdf:resource="https://w3id.org/gfo-light/Relator"/>
        <rdfs:range rdf:resource="https://w3id.org/gfo-light/Continuant"/>
        <rdfs:label xml:lang="en">relates</rdfs:label>
    </owl:ObjectProperty>
    


    <!-- https://w3id.org/gfo-light/representedBy -->


    <owl:ObjectProperty rdf:about="https://w3id.org/gfo-light/representedBy">
        <owl:inverseOf rdf:resource="https://w3id.org/gfo-light/represents"/>
        <rdfs:domain rdf:resource="https://w3id.org/gfo-light/Entity"/>
        <rdfs:range rdf:resource="https://w3id.org/gfo-light/InformationObject"/>
        <rdfs:label xml:lang="en">represented by</rdfs:label>
    </owl:ObjectProperty>
    


    <!-- https://w3id.org/gfo-light/represents -->


    <owl:ObjectProperty rdf:about="https://w3id.org/gfo-light/represents">
        <rdfs:domain rdf:resource="https://w3id.org/gfo-light/InformationObject"/>
        <rdfs:range rdf:resource="https://w3id.org/gfo-light/Entity"/>
        <rdfs:label xml:lang="en">represents</rdfs:label>
    </owl:ObjectProperty>
    


    <!-- https://w3id.org/gfo-light/resultsFrom -->


    <owl:ObjectProperty rdf:about="https://w3id.org/gfo-light/resultsFrom">
        <rdfs:domain>
            <owl:Class>
                <owl:unionOf rdf:parseType="Collection">
                    <rdf:Description rdf:about="https://w3id.org/gfo-light/ProcessualEntity"/>
                    <rdf:Description rdf:about="https://w3id.org/gfo-light/SituationalEntity"/>
                </owl:unionOf>
            </owl:Class>
        </rdfs:domain>
        <rdfs:range>
            <owl:Class>
                <owl:unionOf rdf:parseType="Collection">
                    <rdf:Description rdf:about="https://w3id.org/gfo-light/ProcessualEntity"/>
                    <rdf:Description rdf:about="https://w3id.org/gfo-light/SituationalEntity"/>
                </owl:unionOf>
            </owl:Class>
        </rdfs:range>
        <rdfs:label xml:lang="en">results from</rdfs:label>
    </owl:ObjectProperty>
    


    <!-- https://w3id.org/gfo-light/roleIn -->


    <owl:ObjectProperty rdf:about="https://w3id.org/gfo-light/roleIn">
        <rdfs:domain rdf:resource="https://w3id.org/gfo-light/Role"/>
        <rdfs:range>
            <owl:Class>
                <owl:unionOf rdf:parseType="Collection">
                    <rdf:Description rdf:about="https://w3id.org/gfo-light/Object"/>
                    <rdf:Description rdf:about="https://w3id.org/gfo-light/ObjectAggregate"/>
                    <rdf:Description rdf:about="https://w3id.org/gfo-light/ProcessualEntity"/>
                    <rdf:Description rdf:about="https://w3id.org/gfo-light/Relator"/>
                    <rdf:Description rdf:about="https://w3id.org/gfo-light/SituationalEntity"/>
                </owl:unionOf>
            </owl:Class>
        </rdfs:range>
        <rdfs:label xml:lang="en">role in</rdfs:label>
    </owl:ObjectProperty>
    


    <!-- https://w3id.org/gfo-light/situationPartOf -->


    <owl:ObjectProperty rdf:about="https://w3id.org/gfo-light/situationPartOf">
        <rdfs:subPropertyOf rdf:resource="https://w3id.org/gfo-light/partOf"/>
        <rdfs:domain>
            <owl:Class>
                <owl:unionOf rdf:parseType="Collection">
                    <rdf:Description rdf:about="https://w3id.org/gfo-light/Attributive"/>
                    <rdf:Description rdf:about="https://w3id.org/gfo-light/Situation"/>
                </owl:unionOf>
            </owl:Class>
        </rdfs:domain>
        <rdfs:range rdf:resource="https://w3id.org/gfo-light/Situation"/>
        <rdfs:label xml:lang="en">situation part of</rdfs:label>
    </owl:ObjectProperty>
    


    <!-- https://w3id.org/gfo-light/spatiallyEndsOn -->


    <owl:ObjectProperty rdf:about="https://w3id.org/gfo-light/spatiallyEndsOn">
        <rdfs:subPropertyOf rdf:resource="https://w3id.org/gfo-light/spatiallyPassesThrough"/>
        <rdfs:label xml:lang="en">spatially ends on</rdfs:label>
    </owl:ObjectProperty>
    


    <!-- https://w3id.org/gfo-light/spatiallyPassesThrough -->


    <owl:ObjectProperty rdf:about="https://w3id.org/gfo-light/spatiallyPassesThrough">
        <rdfs:domain>
            <owl:Class>
                <owl:unionOf rdf:parseType="Collection">
                    <rdf:Description rdf:about="https://w3id.org/gfo-light/Line"/>
                    <rdf:Description rdf:about="https://w3id.org/gfo-light/Surface"/>
                </owl:unionOf>
            </owl:Class>
        </rdfs:domain>
        <rdfs:range rdf:resource="https://w3id.org/gfo-light/Continuant"/>
        <rdfs:label xml:lang="en">spatially passes through</rdfs:label>
    </owl:ObjectProperty>
    


    <!-- https://w3id.org/gfo-light/spatiallyStartsOn -->


    <owl:ObjectProperty rdf:about="https://w3id.org/gfo-light/spatiallyStartsOn">
        <rdfs:subPropertyOf rdf:resource="https://w3id.org/gfo-light/spatiallyPassesThrough"/>
        <rdfs:label xml:lang="en">spatially starts on</rdfs:label>
    </owl:ObjectProperty>
    


    <!-- https://w3id.org/gfo-light/temporalPartOf -->


    <owl:ObjectProperty rdf:about="https://w3id.org/gfo-light/temporalPartOf">
        <rdfs:subPropertyOf rdf:resource="https://w3id.org/gfo-light/temporallyRelatedWith"/>
        <rdfs:label xml:lang="en">temporal part of</rdfs:label>
        <skos:definition xml:lang="en">X temporal part of Y: X starts Y or X finishes Y or X during Y</skos:definition>
    </owl:ObjectProperty>
    


    <!-- https://w3id.org/gfo-light/temporallyContains -->


    <owl:ObjectProperty rdf:about="https://w3id.org/gfo-light/temporallyContains">
        <rdfs:subPropertyOf rdf:resource="https://w3id.org/gfo-light/hasTemporalPart"/>
        <rdfs:label xml:lang="en">temporally contains</rdfs:label>
    </owl:ObjectProperty>
    


    <!-- https://w3id.org/gfo-light/temporallyEqual -->


    <owl:ObjectProperty rdf:about="https://w3id.org/gfo-light/temporallyEqual">
        <rdfs:subPropertyOf rdf:resource="https://w3id.org/gfo-light/temporallyRelatedWith"/>
        <rdfs:label xml:lang="en">temporally equal</rdfs:label>
        <skos:definition xml:lang="en">X equal Y: Xs = Ys and Xf = Yf</skos:definition>
    </owl:ObjectProperty>
    


    <!-- https://w3id.org/gfo-light/temporallyFinishedBy -->


    <owl:ObjectProperty rdf:about="https://w3id.org/gfo-light/temporallyFinishedBy">
        <rdfs:subPropertyOf rdf:resource="https://w3id.org/gfo-light/hasTemporalPart"/>
        <owl:inverseOf rdf:resource="https://w3id.org/gfo-light/temporallyFinishes"/>
        <rdfs:label xml:lang="en">temporally finished by</rdfs:label>
    </owl:ObjectProperty>
    


    <!-- https://w3id.org/gfo-light/temporallyFinishes -->


    <owl:ObjectProperty rdf:about="https://w3id.org/gfo-light/temporallyFinishes">
        <rdfs:subPropertyOf rdf:resource="https://w3id.org/gfo-light/temporalPartOf"/>
        <rdfs:label xml:lang="en">temporally finishes</rdfs:label>
        <skos:definition xml:lang="en">X finishes Y: Xs &gt; Ys and Xf = Yf</skos:definition>
    </owl:ObjectProperty>
    


    <!-- https://w3id.org/gfo-light/temporallyMeets -->


    <owl:ObjectProperty rdf:about="https://w3id.org/gfo-light/temporallyMeets">
        <rdfs:subPropertyOf rdf:resource="https://w3id.org/gfo-light/temporallyRelatedWith"/>
        <owl:inverseOf rdf:resource="https://w3id.org/gfo-light/temporallyMetBy"/>
        <rdfs:label xml:lang="en">temporally meets</rdfs:label>
        <skos:definition xml:lang="en">X meets Y: Xf = Ys</skos:definition>
    </owl:ObjectProperty>
    


    <!-- https://w3id.org/gfo-light/temporallyMetBy -->


    <owl:ObjectProperty rdf:about="https://w3id.org/gfo-light/temporallyMetBy">
        <rdfs:subPropertyOf rdf:resource="https://w3id.org/gfo-light/temporallyRelatedWith"/>
        <rdfs:label xml:lang="en">temporally met by</rdfs:label>
    </owl:ObjectProperty>
    


    <!-- https://w3id.org/gfo-light/temporallyOverlappedBy -->


    <owl:ObjectProperty rdf:about="https://w3id.org/gfo-light/temporallyOverlappedBy">
        <rdfs:subPropertyOf rdf:resource="https://w3id.org/gfo-light/temporallyRelatedWith"/>
        <owl:inverseOf rdf:resource="https://w3id.org/gfo-light/temporallyOverlaps"/>
        <rdfs:label xml:lang="en">temporally overlapped by</rdfs:label>
    </owl:ObjectProperty>
    


    <!-- https://w3id.org/gfo-light/temporallyOverlaps -->


    <owl:ObjectProperty rdf:about="https://w3id.org/gfo-light/temporallyOverlaps">
        <rdfs:subPropertyOf rdf:resource="https://w3id.org/gfo-light/temporallyRelatedWith"/>
        <rdfs:label xml:lang="en">temporally overlaps</rdfs:label>
        <skos:definition xml:lang="en">X overlaps Y: Xs &lt; Ys and Xf &gt; Ys and Xf &lt; Yf</skos:definition>
    </owl:ObjectProperty>
    


    <!-- https://w3id.org/gfo-light/temporallyRelatedWith -->


    <owl:ObjectProperty rdf:about="https://w3id.org/gfo-light/temporallyRelatedWith">
        <rdfs:domain rdf:resource="https://w3id.org/gfo-light/Individual"/>
        <rdfs:range rdf:resource="https://w3id.org/gfo-light/Individual"/>
        <rdfs:comment xml:lang="en">If a temporal relation is applied to other concrete individuals as time intervals (attributive, continuant, process, situation), it is propagated to their existence times (hasTime).</rdfs:comment>
        <rdfs:comment xml:lang="en">In the definitions of the relations, the variables Xs, Xf, Ys and Yf represent the start (s) and finish (f) of the time intervals X and Y.</rdfs:comment>
        <rdfs:comment xml:lang="en">Some temporal relations can also be applied to points in time (before/after, equal) or a point in time and a time interval (before, starts, finishes, during or their inverse relations).</rdfs:comment>
        <rdfs:label xml:lang="en">temporally related with</rdfs:label>
        <skos:definition xml:lang="en">Temporal relations between time intervals based on Allen, J. F. (1983). Maintaining knowledge about temporal intervals. Communications of the ACM, 26(11), 832-843.</skos:definition>
    </owl:ObjectProperty>
    


    <!-- https://w3id.org/gfo-light/temporallyStartedBy -->


    <owl:ObjectProperty rdf:about="https://w3id.org/gfo-light/temporallyStartedBy">
        <rdfs:subPropertyOf rdf:resource="https://w3id.org/gfo-light/hasTemporalPart"/>
        <owl:inverseOf rdf:resource="https://w3id.org/gfo-light/temporallyStarts"/>
        <rdfs:label xml:lang="en">temporally started by</rdfs:label>
    </owl:ObjectProperty>
    


    <!-- https://w3id.org/gfo-light/temporallyStarts -->


    <owl:ObjectProperty rdf:about="https://w3id.org/gfo-light/temporallyStarts">
        <rdfs:subPropertyOf rdf:resource="https://w3id.org/gfo-light/temporalPartOf"/>
        <rdfs:label xml:lang="en">temporally starts</rdfs:label>
        <skos:definition xml:lang="en">X starts Y: Xs = Ys and Xf &lt; Yf</skos:definition>
    </owl:ObjectProperty>
    


    <!-- https://w3id.org/gfo-light/timeOf -->


    <owl:ObjectProperty rdf:about="https://w3id.org/gfo-light/timeOf">
        <rdfs:domain rdf:resource="https://w3id.org/gfo-light/TimeEntity"/>
        <rdfs:range rdf:resource="https://w3id.org/gfo-light/ConcreteIndividual"/>
        <rdfs:label xml:lang="en">time of</rdfs:label>
    </owl:ObjectProperty>
    


    <!-- 
    ///////////////////////////////////////////////////////////////////////////////////////
    //
    // Data properties
    //
    ///////////////////////////////////////////////////////////////////////////////////////
     -->


    


    <!-- https://w3id.org/gfo-light/afterDateTimeValue -->


    <owl:DatatypeProperty rdf:about="https://w3id.org/gfo-light/afterDateTimeValue">
        <rdfs:subPropertyOf rdf:resource="https://w3id.org/gfo-light/dateTimeValue"/>
        <rdfs:comment xml:lang="en">Shortcut for &apos;after&apos;</rdfs:comment>
        <rdfs:label xml:lang="en">after date time value</rdfs:label>
    </owl:DatatypeProperty>
    


    <!-- https://w3id.org/gfo-light/beforeDateTimeValue -->


    <owl:DatatypeProperty rdf:about="https://w3id.org/gfo-light/beforeDateTimeValue">
        <rdfs:subPropertyOf rdf:resource="https://w3id.org/gfo-light/dateTimeValue"/>
        <rdfs:comment xml:lang="en">Shortcut for &apos;before&apos;</rdfs:comment>
        <rdfs:label xml:lang="en">before date time value</rdfs:label>
    </owl:DatatypeProperty>
    


    <!-- https://w3id.org/gfo-light/booleanValue -->


    <owl:DatatypeProperty rdf:about="https://w3id.org/gfo-light/booleanValue">
        <rdfs:domain rdf:resource="https://w3id.org/gfo-light/Attributive"/>
        <rdfs:range rdf:resource="http://www.w3.org/2001/XMLSchema#boolean"/>
        <rdfs:label xml:lang="en">boolean value</rdfs:label>
    </owl:DatatypeProperty>
    


    <!-- https://w3id.org/gfo-light/containsDateTimeValue -->


    <owl:DatatypeProperty rdf:about="https://w3id.org/gfo-light/containsDateTimeValue">
        <rdfs:subPropertyOf rdf:resource="https://w3id.org/gfo-light/hasTemporalPartDateTimeValue"/>
        <rdfs:comment xml:lang="en">Shortcut for &apos;temporallyContains&apos;</rdfs:comment>
        <rdfs:label xml:lang="en">contains date time value</rdfs:label>
    </owl:DatatypeProperty>
    


    <!-- https://w3id.org/gfo-light/dateTimeValue -->


    <owl:DatatypeProperty rdf:about="https://w3id.org/gfo-light/dateTimeValue">
        <rdfs:domain rdf:resource="https://w3id.org/gfo-light/Individual"/>
        <rdfs:range rdf:resource="http://www.w3.org/2001/XMLSchema#dateTime"/>
        <rdfs:label xml:lang="en">date time value</rdfs:label>
    </owl:DatatypeProperty>
    


    <!-- https://w3id.org/gfo-light/decimalValue -->


    <owl:DatatypeProperty rdf:about="https://w3id.org/gfo-light/decimalValue">
        <rdfs:domain rdf:resource="https://w3id.org/gfo-light/Attributive"/>
        <rdfs:range rdf:resource="http://www.w3.org/2001/XMLSchema#decimal"/>
        <rdfs:label xml:lang="en">decimal value</rdfs:label>
    </owl:DatatypeProperty>
    


    <!-- https://w3id.org/gfo-light/finishedByDateTimeValue -->


    <owl:DatatypeProperty rdf:about="https://w3id.org/gfo-light/finishedByDateTimeValue">
        <rdfs:subPropertyOf rdf:resource="https://w3id.org/gfo-light/hasTemporalPartDateTimeValue"/>
        <rdfs:comment xml:lang="en">Shortcut for &apos;temporallyFinishedBy&apos;</rdfs:comment>
        <rdfs:label xml:lang="en">finished by date time value</rdfs:label>
    </owl:DatatypeProperty>
    


    <!-- https://w3id.org/gfo-light/hasTemporalPartDateTimeValue -->


    <owl:DatatypeProperty rdf:about="https://w3id.org/gfo-light/hasTemporalPartDateTimeValue">
        <rdfs:subPropertyOf rdf:resource="https://w3id.org/gfo-light/dateTimeValue"/>
        <rdfs:comment xml:lang="en">Shortcut for &apos;hasTemporalPart&apos;</rdfs:comment>
        <rdfs:label xml:lang="en">has temporal part date time value</rdfs:label>
    </owl:DatatypeProperty>
    


    <!-- https://w3id.org/gfo-light/startedByDateTimeValue -->


    <owl:DatatypeProperty rdf:about="https://w3id.org/gfo-light/startedByDateTimeValue">
        <rdfs:subPropertyOf rdf:resource="https://w3id.org/gfo-light/hasTemporalPartDateTimeValue"/>
        <rdfs:comment xml:lang="en">Shortcut for &apos;temporallyStartedBy&apos;</rdfs:comment>
        <rdfs:label xml:lang="en">started by date time value</rdfs:label>
    </owl:DatatypeProperty>
    


    <!-- https://w3id.org/gfo-light/stringValue -->


    <owl:DatatypeProperty rdf:about="https://w3id.org/gfo-light/stringValue">
        <rdfs:domain rdf:resource="https://w3id.org/gfo-light/Attributive"/>
        <rdfs:range rdf:resource="http://www.w3.org/2001/XMLSchema#string"/>
        <rdfs:label xml:lang="en">string value</rdfs:label>
    </owl:DatatypeProperty>
    


    <!-- https://w3id.org/gfo-light/unit -->


    <owl:DatatypeProperty rdf:about="https://w3id.org/gfo-light/unit">
        <rdfs:domain rdf:resource="https://w3id.org/gfo-light/Attributive"/>
        <rdfs:range rdf:resource="http://www.w3.org/2001/XMLSchema#string"/>
        <rdfs:label xml:lang="en">unit</rdfs:label>
    </owl:DatatypeProperty>
    


    <!-- 
    ///////////////////////////////////////////////////////////////////////////////////////
    //
    // Classes
    //
    ///////////////////////////////////////////////////////////////////////////////////////
     -->


    


    <!-- https://w3id.org/cop/Algorithm -->


    <owl:Class rdf:about="https://w3id.org/cop/Algorithm">
        <rdfs:subClassOf rdf:resource="https://w3id.org/gfo-light/InformationObject"/>
        <rdfs:subClassOf>
            <owl:Restriction>
                <owl:onProperty rdf:resource="https://w3id.org/cop/implementedBy"/>
                <owl:allValuesFrom rdf:resource="https://w3id.org/cop/Software"/>
            </owl:Restriction>
        </rdfs:subClassOf>
        <rdfs:label xml:lang="en">Algorithm</rdfs:label>
        <rdfs:label xml:lang="de">Algorithmus</rdfs:label>
        <skos:definition xml:lang="en">An algorithm is a specification of instructions to solve a problem or a class of problems.</skos:definition>
        <skos:definition xml:lang="de">Ein Algorithmus ist eine Spezifikation von Anweisungen zur Lösung eines Problems oder einer Klasse von Problemen.</skos:definition>
    </owl:Class>
    


    <!-- https://w3id.org/cop/AttributeSpec -->


    <owl:Class rdf:about="https://w3id.org/cop/AttributeSpec">
        <rdfs:subClassOf rdf:resource="https://w3id.org/gfo-light/InformationObject"/>
        <rdfs:subClassOf>
            <owl:Restriction>
                <owl:onProperty rdf:resource="https://w3id.org/gfo-light/partOf"/>
                <owl:someValuesFrom rdf:resource="https://w3id.org/cop/PhenotypeClassView"/>
            </owl:Restriction>
        </rdfs:subClassOf>
        <rdfs:label xml:lang="en">Attribute specification</rdfs:label>
        <rdfs:label xml:lang="de">Attributspezifikation</rdfs:label>
        <skos:definition xml:lang="en">An attribute specification is a specification of an attribute.</skos:definition>
        <skos:definition xml:lang="de">Eine Attributspezifikation ist eine Spezifikation eines Attributs.</skos:definition>
    </owl:Class>
    


    <!-- https://w3id.org/cop/BasicRestrictedPhenotypeClassView -->


    <owl:Class rdf:about="https://w3id.org/cop/BasicRestrictedPhenotypeClassView">
        <rdfs:subClassOf rdf:resource="https://w3id.org/cop/PhenotypeClassView"/>
        <rdfs:subClassOf>
            <owl:Restriction>
                <owl:onProperty rdf:resource="https://w3id.org/cop/basicRestrictionOf"/>
                <owl:qualifiedCardinality rdf:datatype="http://www.w3.org/2001/XMLSchema#nonNegativeInteger">1</owl:qualifiedCardinality>
                <owl:onClass rdf:resource="https://w3id.org/cop/BasicUnrestrictedPhenotypeClassView"/>
            </owl:Restriction>
        </rdfs:subClassOf>
        <rdfs:subClassOf>
            <owl:Restriction>
                <owl:onProperty rdf:resource="https://w3id.org/gfo-light/hasPart"/>
                <owl:qualifiedCardinality rdf:datatype="http://www.w3.org/2001/XMLSchema#nonNegativeInteger">1</owl:qualifiedCardinality>
                <owl:onClass rdf:resource="https://w3id.org/cop/ValueRangeSpec"/>
            </owl:Restriction>
        </rdfs:subClassOf>
        <rdfs:subClassOf>
            <owl:Restriction>
                <owl:onProperty rdf:resource="https://w3id.org/gfo-light/represents"/>
                <owl:qualifiedCardinality rdf:datatype="http://www.w3.org/2001/XMLSchema#nonNegativeInteger">1</owl:qualifiedCardinality>
                <owl:onClass rdf:resource="https://w3id.org/cop/RestrictedPhenotypeClass"/>
            </owl:Restriction>
        </rdfs:subClassOf>
        <rdfs:label xml:lang="en">Basic restricted phenotype class view</rdfs:label>
        <rdfs:label xml:lang="de">Basissicht einer eingeschränkten Phänotypklasse</rdfs:label>
        <skos:definition xml:lang="en">A basic restricted phenotype class view represents a restricted phenotype class that restricts an unrestricted phenotype class represented by a basic view.</skos:definition>
        <skos:definition xml:lang="de">Eine Basissicht einer eingeschränkten Phänotypklasse repräsentiert eine eingeschränkte Phänotypklasse, die eine uneingeschränkte Phänotypklasse einschränkt, die durch eine Basissicht repräsentiert wird.</skos:definition>
        <skos:example xml:lang="en">Specification of the phenotype class &apos;Weight over 100 kg&apos;</skos:example>
    </owl:Class>
    


    <!-- https://w3id.org/cop/BasicUnrestrictedPhenotypeClassView -->


    <owl:Class rdf:about="https://w3id.org/cop/BasicUnrestrictedPhenotypeClassView">
        <rdfs:subClassOf rdf:resource="https://w3id.org/cop/PhenotypeClassView"/>
        <rdfs:subClassOf>
            <owl:Restriction>
                <owl:onProperty rdf:resource="https://w3id.org/gfo-light/hasPart"/>
                <owl:someValuesFrom rdf:resource="https://w3id.org/cop/TerminologyCode"/>
            </owl:Restriction>
        </rdfs:subClassOf>
        <rdfs:subClassOf>
            <owl:Restriction>
                <owl:onProperty rdf:resource="https://w3id.org/gfo-light/hasPart"/>
                <owl:qualifiedCardinality rdf:datatype="http://www.w3.org/2001/XMLSchema#nonNegativeInteger">1</owl:qualifiedCardinality>
                <owl:onClass rdf:resource="https://w3id.org/cop/DataTypeSpec"/>
            </owl:Restriction>
        </rdfs:subClassOf>
        <rdfs:subClassOf>
            <owl:Restriction>
                <owl:onProperty rdf:resource="https://w3id.org/gfo-light/represents"/>
                <owl:qualifiedCardinality rdf:datatype="http://www.w3.org/2001/XMLSchema#nonNegativeInteger">1</owl:qualifiedCardinality>
                <owl:onClass rdf:resource="https://w3id.org/cop/UnrestrictedPhenotypeClass"/>
            </owl:Restriction>
        </rdfs:subClassOf>
        <rdfs:label xml:lang="en">Basic unrestricted phenotype class view</rdfs:label>
        <rdfs:label xml:lang="de">Basissicht einer uneingeschränkten Phänotypklasse</rdfs:label>
        <skos:definition xml:lang="en">A basic unrestricted phenotype class view represents an unrestricted phenotype class whose instances (phenotypes) have already been determined and can be queried from the data source.</skos:definition>
        <skos:definition xml:lang="de">Eine Basissicht einer uneingeschränkten Phänotypklasse repräsentiert eine uneingeschränkte Phänotypklasse, deren Instanzen (Phänotypen) bereits bestimmt wurden und von der Datenquelle abgefragt werden können.</skos:definition>
        <skos:example xml:lang="en">Specification of the phenotype class &apos;Weight&apos;</skos:example>
    </owl:Class>
    


    <!-- https://w3id.org/cop/BooleanSpec -->


    <owl:Class rdf:about="https://w3id.org/cop/BooleanSpec">
        <rdfs:subClassOf rdf:resource="https://w3id.org/cop/DataTypeSpec"/>
        <rdfs:label xml:lang="en">Boolean data type specification</rdfs:label>
    </owl:Class>
    


    <!-- https://w3id.org/cop/DataTypeSpec -->


    <owl:Class rdf:about="https://w3id.org/cop/DataTypeSpec">
        <rdfs:subClassOf rdf:resource="https://w3id.org/cop/AttributeSpec"/>
        <rdfs:label xml:lang="en">Data type specification</rdfs:label>
        <rdfs:label xml:lang="de">Datentypspezifikation</rdfs:label>
        <skos:definition xml:lang="en">A data type specification is a specification of a data type (e.g., string, decimal, boolean or date-time).</skos:definition>
        <skos:definition xml:lang="de">Eine Datentypspezifikation ist eine Spezifikation eines Datentyps (z.B. Text, Zahl, Boolescher Wert oder Datum-Uhrzeit).</skos:definition>
    </owl:Class>
    


    <!-- https://w3id.org/cop/DateTimeSpec -->


    <owl:Class rdf:about="https://w3id.org/cop/DateTimeSpec">
        <rdfs:subClassOf rdf:resource="https://w3id.org/cop/DataTypeSpec"/>
        <rdfs:label xml:lang="en">Date-time data type specification</rdfs:label>
    </owl:Class>
    


    <!-- https://w3id.org/cop/DecimalSpec -->


    <owl:Class rdf:about="https://w3id.org/cop/DecimalSpec">
        <rdfs:subClassOf rdf:resource="https://w3id.org/cop/DataTypeSpec"/>
        <rdfs:label xml:lang="en">Decimal data type specification</rdfs:label>
    </owl:Class>
    


    <!-- https://w3id.org/cop/DerivationExpression -->


    <owl:Class rdf:about="https://w3id.org/cop/DerivationExpression">
        <rdfs:subClassOf rdf:resource="https://w3id.org/cop/AttributeSpec"/>
        <rdfs:subClassOf>
            <owl:Restriction>
                <owl:onProperty rdf:resource="https://w3id.org/cop/hasVariable"/>
                <owl:someValuesFrom rdf:resource="https://w3id.org/cop/PhenotypeClassView"/>
            </owl:Restriction>
        </rdfs:subClassOf>
        <rdfs:subClassOf>
            <owl:Restriction>
                <owl:onProperty rdf:resource="https://w3id.org/gfo-light/partOf"/>
                <owl:someValuesFrom rdf:resource="https://w3id.org/cop/DerivedUnrestrictedPhenotypeClassView"/>
            </owl:Restriction>
        </rdfs:subClassOf>
        <rdfs:label xml:lang="de">Ableitungsausdruck</rdfs:label>
        <rdfs:label xml:lang="en">Derivation expression</rdfs:label>
        <skos:definition xml:lang="en">A derivation expression is an executable formal specification of a combination of different functions/operators and input variables, the execution of which calculates/derives a new value (e.g., of a phenotype) based on the input values.</skos:definition>
        <skos:definition xml:lang="de">Ein Ableitungsausdruck ist eine ausführbare formale Spezifikation einer Kombination aus verschiedenen Funktionen/Operatoren und Eingabevariablen, deren Ausführung einen neuen Wert (z.B. eines Phänotyps) auf der Grundlage der Eingabewerte berechnet/ableitet.</skos:definition>
    </owl:Class>
    


    <!-- https://w3id.org/cop/DerivedRestrictedPhenotypeClassView -->


    <owl:Class rdf:about="https://w3id.org/cop/DerivedRestrictedPhenotypeClassView">
        <rdfs:subClassOf rdf:resource="https://w3id.org/cop/PhenotypeClassView"/>
        <rdfs:subClassOf>
            <owl:Restriction>
                <owl:onProperty rdf:resource="https://w3id.org/cop/derivedRestrictionOf"/>
                <owl:qualifiedCardinality rdf:datatype="http://www.w3.org/2001/XMLSchema#nonNegativeInteger">1</owl:qualifiedCardinality>
                <owl:onClass rdf:resource="https://w3id.org/cop/DerivedUnrestrictedPhenotypeClassView"/>
            </owl:Restriction>
        </rdfs:subClassOf>
        <rdfs:subClassOf>
            <owl:Restriction>
                <owl:onProperty rdf:resource="https://w3id.org/gfo-light/hasPart"/>
                <owl:qualifiedCardinality rdf:datatype="http://www.w3.org/2001/XMLSchema#nonNegativeInteger">1</owl:qualifiedCardinality>
                <owl:onClass rdf:resource="https://w3id.org/cop/ValueRangeSpec"/>
            </owl:Restriction>
        </rdfs:subClassOf>
        <rdfs:subClassOf>
            <owl:Restriction>
                <owl:onProperty rdf:resource="https://w3id.org/gfo-light/represents"/>
                <owl:qualifiedCardinality rdf:datatype="http://www.w3.org/2001/XMLSchema#nonNegativeInteger">1</owl:qualifiedCardinality>
                <owl:onClass rdf:resource="https://w3id.org/cop/RestrictedPhenotypeClass"/>
            </owl:Restriction>
        </rdfs:subClassOf>
        <rdfs:label xml:lang="de">Ableitungssicht einer eingeschränkten Phänotypklasse</rdfs:label>
        <rdfs:label xml:lang="en">Derived restricted phenotype class view</rdfs:label>
        <skos:definition xml:lang="en">A derived restricted phenotype class view represents a restricted phenotype class that restricts an unrestricted phenotype class represented by a derived view.</skos:definition>
        <skos:definition xml:lang="de">Eine Ableitungssicht einer eingeschränkten Phänotypklasse repräsentiert eine eingeschränkte Phänotypklasse, die eine uneingeschränkte Phänotypklasse einschränkt, die durch eine Ableitungssicht repräsentiert wird.</skos:definition>
        <skos:example xml:lang="en">Specification of the phenotype class &apos;Overweight (e.g., BMI over 30)&apos;</skos:example>
    </owl:Class>
    


    <!-- https://w3id.org/cop/DerivedUnrestrictedPhenotypeClassView -->


    <owl:Class rdf:about="https://w3id.org/cop/DerivedUnrestrictedPhenotypeClassView">
        <rdfs:subClassOf rdf:resource="https://w3id.org/cop/PhenotypeClassView"/>
        <rdfs:subClassOf>
            <owl:Restriction>
                <owl:onProperty rdf:resource="https://w3id.org/cop/derivedFrom"/>
                <owl:someValuesFrom rdf:resource="https://w3id.org/cop/PhenotypeClassView"/>
            </owl:Restriction>
        </rdfs:subClassOf>
        <rdfs:subClassOf>
            <owl:Restriction>
                <owl:onProperty rdf:resource="https://w3id.org/gfo-light/hasPart"/>
                <owl:qualifiedCardinality rdf:datatype="http://www.w3.org/2001/XMLSchema#nonNegativeInteger">1</owl:qualifiedCardinality>
                <owl:onClass rdf:resource="https://w3id.org/cop/DerivationExpression"/>
            </owl:Restriction>
        </rdfs:subClassOf>
        <rdfs:subClassOf>
            <owl:Restriction>
                <owl:onProperty rdf:resource="https://w3id.org/gfo-light/represents"/>
                <owl:qualifiedCardinality rdf:datatype="http://www.w3.org/2001/XMLSchema#nonNegativeInteger">1</owl:qualifiedCardinality>
                <owl:onClass rdf:resource="https://w3id.org/cop/UnrestrictedPhenotypeClass"/>
            </owl:Restriction>
        </rdfs:subClassOf>
        <rdfs:label xml:lang="de">Ableitungssicht einer uneingeschränkten Phänotypklasse</rdfs:label>
        <rdfs:label xml:lang="en">Derived unrestricted phenotype class view</rdfs:label>
        <skos:definition xml:lang="en">A derived unrestricted phenotype class view represents an unrestricted phenotype class whose instances (phenotypes) need to be determined (i.e., derived from other phenotypes).</skos:definition>
        <skos:definition xml:lang="de">Eine Ableitungssicht einer uneingeschränkten Phänotypklasse repräsentiert eine uneingeschränkte Phänotypklasse, deren Instanzen (Phänotypen) bestimmt (d.h. von anderen Phänotypen abgeleitet) werden müssen.</skos:definition>
        <skos:example xml:lang="en">Specification of the phenotype class &apos;Body Mass Index (BMI)&apos;</skos:example>
    </owl:Class>
    


    <!-- https://w3id.org/cop/Description -->


    <owl:Class rdf:about="https://w3id.org/cop/Description">
        <rdfs:subClassOf rdf:resource="https://w3id.org/cop/AttributeSpec"/>
        <rdfs:label xml:lang="de">Beschreibung</rdfs:label>
        <rdfs:label xml:lang="en">Description</rdfs:label>
        <skos:definition xml:lang="en">A description is a string describing an entity.</skos:definition>
        <skos:definition xml:lang="de">Eine Beschreibung ist eine Zeichenkette, die eine Entität beschreibt.</skos:definition>
    </owl:Class>
    


    <!-- https://w3id.org/cop/DynamicPhenotypeAlgorithm -->


    <owl:Class rdf:about="https://w3id.org/cop/DynamicPhenotypeAlgorithm">
        <rdfs:subClassOf rdf:resource="https://w3id.org/cop/PhenotypeAlgorithm"/>
        <rdfs:label xml:lang="en">Dynamic phenotype algorithm</rdfs:label>
        <rdfs:label xml:lang="de">Dynamischer Phänotypalgorithmus</rdfs:label>
        <skos:definition xml:lang="en">A dynamic phenotype algorithm is a phenotype algorithm for executing an arbitrary phenotype query.</skos:definition>
        <skos:definition xml:lang="de">Ein dynamischer Phänotypalgorithmus ist ein Phänotypalgorithmus für die Ausführung einer beliebigen Phänotypabfrage.</skos:definition>
    </owl:Class>
    


    <!-- https://w3id.org/cop/Model -->


    <owl:Class rdf:about="https://w3id.org/cop/Model">
        <rdfs:subClassOf rdf:resource="https://w3id.org/gfo-light/InformationObject"/>
        <rdfs:label xml:lang="en">Model</rdfs:label>
        <rdfs:label xml:lang="de">Modell</rdfs:label>
        <skos:definition xml:lang="en">A model is a representation/specification of an abstraction of an entity.</skos:definition>
        <skos:definition xml:lang="de">Ein Modell ist eine Repräsentation/Spezifikation einer Abstraktion einer Entität.</skos:definition>
    </owl:Class>
    


    <!-- https://w3id.org/cop/Organism -->


    <owl:Class rdf:about="https://w3id.org/cop/Organism">
        <rdfs:subClassOf rdf:resource="https://w3id.org/gfo-light/Object"/>
        <rdfs:subClassOf>
            <owl:Restriction>
                <owl:onProperty rdf:resource="https://w3id.org/gfo-light/hasAttributive"/>
                <owl:someValuesFrom rdf:resource="https://w3id.org/cop/Phenotype"/>
            </owl:Restriction>
        </rdfs:subClassOf>
        <rdfs:label xml:lang="en">Organism</rdfs:label>
        <rdfs:label xml:lang="de">Organismus</rdfs:label>
        <skos:definition xml:lang="en">An organism is a living object.</skos:definition>
        <skos:definition xml:lang="de">Ein Organismus ist ein lebendes Objekt.</skos:definition>
    </owl:Class>
    


    <!-- https://w3id.org/cop/Phenotype -->


    <owl:Class rdf:about="https://w3id.org/cop/Phenotype">
        <rdfs:subClassOf rdf:resource="https://w3id.org/gfo-light/Attributive"/>
        <rdfs:subClassOf>
            <owl:Restriction>
                <owl:onProperty rdf:resource="https://w3id.org/gfo-light/instanceOf"/>
                <owl:someValuesFrom rdf:resource="https://w3id.org/cop/PhenotypeClass"/>
            </owl:Restriction>
        </rdfs:subClassOf>
        <rdfs:subClassOf>
            <owl:Restriction>
                <owl:onProperty rdf:resource="https://w3id.org/gfo-light/attributiveOf"/>
                <owl:qualifiedCardinality rdf:datatype="http://www.w3.org/2001/XMLSchema#nonNegativeInteger">1</owl:qualifiedCardinality>
                <owl:onClass rdf:resource="https://w3id.org/cop/Organism"/>
            </owl:Restriction>
        </rdfs:subClassOf>
        <rdfs:label xml:lang="en">Phenotype</rdfs:label>
        <rdfs:label xml:lang="de">Phänotyp</rdfs:label>
        <skos:definition xml:lang="en">A phenotype is a (combination of) bodily feature(s) or observable characteristic(s)/trait(s) of an organism.</skos:definition>
        <skos:definition xml:lang="de">Ein Phänotyp ist eine (Kombination von) körperliche(n) Eigenschaft(en) oder beobachtbare(s) Merkmal(e)/Eigenschaft(en) eines Organismus.</skos:definition>
        <skos:example xml:lang="en">Body Mass Index (BMI) of a specific person</skos:example>
        <skos:example xml:lang="en">Overweight of a specific person</skos:example>
        <skos:example xml:lang="en">Weight of a specific person</skos:example>
    </owl:Class>
    <owl:Axiom>
        <owl:annotatedSource rdf:resource="https://w3id.org/cop/Phenotype"/>
        <owl:annotatedProperty rdf:resource="http://www.w3.org/2004/02/skos/core#definition"/>
        <owl:annotatedTarget xml:lang="en">A phenotype is a (combination of) bodily feature(s) or observable characteristic(s)/trait(s) of an organism.</owl:annotatedTarget>
        <terms:references xml:lang="en">Mahner M, Kary M. What Exactly Are Genomes, Genotypes and Phenotypes? And What About Phenomes? J Theor Biol 1997;186:55–63. https://doi.org/10.1006/jtbi.1996.0335.</terms:references>
        <terms:references xml:lang="en">Scheuermann RH, Ceusters W, Smith B. Toward an Ontological Treatment of Disease and Diagnosis. Summit Transl Bioinforma 2009;2009:116–20. https://pmc.ncbi.nlm.nih.gov/articles/PMC3041577/</terms:references>
    </owl:Axiom>
    


    <!-- https://w3id.org/cop/PhenotypeAlgorithm -->


    <owl:Class rdf:about="https://w3id.org/cop/PhenotypeAlgorithm">
        <rdfs:subClassOf rdf:resource="https://w3id.org/cop/Algorithm"/>
        <rdfs:subClassOf>
            <owl:Restriction>
                <owl:onProperty rdf:resource="https://w3id.org/cop/applicableFor"/>
                <owl:someValuesFrom rdf:resource="https://w3id.org/cop/PhenotypeQuery"/>
            </owl:Restriction>
        </rdfs:subClassOf>
        <rdfs:subClassOf>
            <owl:Restriction>
                <owl:onProperty rdf:resource="https://w3id.org/cop/implementedBy"/>
                <owl:allValuesFrom rdf:resource="https://w3id.org/cop/PhenotypingSoftware"/>
            </owl:Restriction>
        </rdfs:subClassOf>
        <rdfs:label xml:lang="en">Phenotype algorithm</rdfs:label>
        <rdfs:label xml:lang="de">Phänotypalgorithmus</rdfs:label>
        <skos:definition xml:lang="en">A phenotype algorithm is an algorithm for executing a phenotype query, i.e., identifying individuals matching the query criteria (i.e., meeting all the inclusion but none of the exclusion criteria) and deriving/outputting further phenotypes (projection entries).</skos:definition>
        <skos:definition xml:lang="de">Ein Phänotypalgorithmus ist ein Algorithmus zur Ausführung einer Phänotypabfrage, d.h. zur Identifizierung von Individuen, die den Abfragekriterien entsprechen (d.h. alle Einschluss-, aber keines der Ausschlusskriterien erfüllen) und zur Ableitung/Ausgabe weiterer Phänotypen (Projektionseinträge).</skos:definition>
    </owl:Class>
    


    <!-- https://w3id.org/cop/PhenotypeClass -->


    <owl:Class rdf:about="https://w3id.org/cop/PhenotypeClass">
        <rdfs:subClassOf rdf:resource="https://w3id.org/gfo-light/Category"/>
        <rdfs:subClassOf>
            <owl:Restriction>
                <owl:onProperty rdf:resource="https://w3id.org/gfo-light/instantiatedBy"/>
                <owl:allValuesFrom rdf:resource="https://w3id.org/cop/Phenotype"/>
            </owl:Restriction>
        </rdfs:subClassOf>
        <owl:disjointUnionOf rdf:parseType="Collection">
            <rdf:Description rdf:about="https://w3id.org/cop/RestrictedPhenotypeClass"/>
            <rdf:Description rdf:about="https://w3id.org/cop/UnrestrictedPhenotypeClass"/>
        </owl:disjointUnionOf>
        <rdfs:label xml:lang="en">Phenotype class</rdfs:label>
        <rdfs:label xml:lang="de">Phänotypklasse</rdfs:label>
        <skos:definition xml:lang="en">Phenotype classes are categories whose instances are phenotypes.</skos:definition>
        <skos:definition xml:lang="de">Phänotypklassen sind Kategorien, deren Instanzen Phänotypen sind.</skos:definition>
    </owl:Class>
    


    <!-- https://w3id.org/cop/PhenotypeClassView -->


    <owl:Class rdf:about="https://w3id.org/cop/PhenotypeClassView">
        <rdfs:subClassOf rdf:resource="https://w3id.org/cop/Model"/>
        <rdfs:subClassOf>
            <owl:Restriction>
                <owl:onProperty rdf:resource="https://w3id.org/gfo-light/hasPart"/>
                <owl:someValuesFrom rdf:resource="https://w3id.org/cop/Title"/>
            </owl:Restriction>
        </rdfs:subClassOf>
        <rdfs:subClassOf>
            <owl:Restriction>
                <owl:onProperty rdf:resource="https://w3id.org/gfo-light/represents"/>
                <owl:qualifiedCardinality rdf:datatype="http://www.w3.org/2001/XMLSchema#nonNegativeInteger">1</owl:qualifiedCardinality>
                <owl:onClass rdf:resource="https://w3id.org/cop/PhenotypeClass"/>
            </owl:Restriction>
        </rdfs:subClassOf>
        <rdfs:label xml:lang="en">Phenotype class view</rdfs:label>
        <rdfs:label xml:lang="de">Phänotypklassensicht</rdfs:label>
        <skos:definition xml:lang="en">A phenotype class view is a formal representation of a phenotype class (its attributes and relationships).</skos:definition>
        <skos:definition xml:lang="de">Eine Phänotypklassensicht ist eine formale Repräsentation einer Phänotypklasse (ihrer Attribute und Relationen).</skos:definition>
    </owl:Class>
    


    <!-- https://w3id.org/cop/PhenotypeModel -->


    <owl:Class rdf:about="https://w3id.org/cop/PhenotypeModel">
        <rdfs:subClassOf rdf:resource="https://w3id.org/cop/Model"/>
        <rdfs:subClassOf>
            <owl:Restriction>
                <owl:onProperty rdf:resource="https://w3id.org/gfo-light/hasPart"/>
                <owl:someValuesFrom rdf:resource="https://w3id.org/cop/PhenotypeClassView"/>
            </owl:Restriction>
        </rdfs:subClassOf>
        <rdfs:label xml:lang="en">Phenotype model</rdfs:label>
        <rdfs:label xml:lang="de">Phänotypmodell</rdfs:label>
        <skos:definition xml:lang="en">A phenotype model is a formal representation of delimited phenotypic knowledge (i.e., phenotype classes, their attributes, and relationships).</skos:definition>
        <skos:definition xml:lang="de">Ein Phänotypmodell ist eine formale Darstellung von abgegrenztem phänotypischem Wissen (d.h. von Phänotypklassen, ihren Attributen und Beziehungen).</skos:definition>
    </owl:Class>
    


    <!-- https://w3id.org/cop/PhenotypeQuery -->


    <owl:Class rdf:about="https://w3id.org/cop/PhenotypeQuery">
        <rdfs:subClassOf rdf:resource="https://w3id.org/cop/Model"/>
        <rdfs:subClassOf>
            <owl:Class>
                <owl:unionOf rdf:parseType="Collection">
                    <owl:Restriction>
                        <owl:onProperty rdf:resource="https://w3id.org/cop/hasExclusion"/>
                        <owl:someValuesFrom rdf:resource="https://w3id.org/cop/PhenotypeClassView"/>
                    </owl:Restriction>
                    <owl:Restriction>
                        <owl:onProperty rdf:resource="https://w3id.org/cop/hasInclusion"/>
                        <owl:someValuesFrom rdf:resource="https://w3id.org/cop/PhenotypeClassView"/>
                    </owl:Restriction>
                    <owl:Restriction>
                        <owl:onProperty rdf:resource="https://w3id.org/cop/hasProjection"/>
                        <owl:someValuesFrom rdf:resource="https://w3id.org/cop/PhenotypeClassView"/>
                    </owl:Restriction>
                </owl:unionOf>
            </owl:Class>
        </rdfs:subClassOf>
        <rdfs:subClassOf>
            <owl:Restriction>
                <owl:onProperty rdf:resource="https://w3id.org/cop/basedOn"/>
                <owl:qualifiedCardinality rdf:datatype="http://www.w3.org/2001/XMLSchema#nonNegativeInteger">1</owl:qualifiedCardinality>
                <owl:onClass rdf:resource="https://w3id.org/cop/PhenotypeModel"/>
            </owl:Restriction>
        </rdfs:subClassOf>
        <rdfs:label xml:lang="en">Phenotype query</rdfs:label>
        <rdfs:label xml:lang="de">Phänotypabfrage</rdfs:label>
        <skos:definition xml:lang="en">A phenotype query is a specification of certain phenotype classes as inclusion or exclusion criteria or as projection (output) entries.</skos:definition>
        <skos:definition xml:lang="de">Eine Phänotypabfrage ist eine Spezifikation bestimmter Phänotypklassen als Ein- oder Ausschlusskriterien oder als Projektions- (Ausgabe-) Einträge.</skos:definition>
    </owl:Class>
    


    <!-- https://w3id.org/cop/Phenotyping -->


    <owl:Class rdf:about="https://w3id.org/cop/Phenotyping">
        <rdfs:subClassOf rdf:resource="https://w3id.org/gfo-light/Process"/>
        <rdfs:subClassOf>
            <owl:Restriction>
                <owl:onProperty rdf:resource="https://w3id.org/cop/identifies"/>
                <owl:allValuesFrom rdf:resource="https://w3id.org/cop/Organism"/>
            </owl:Restriction>
        </rdfs:subClassOf>
        <rdfs:label xml:lang="en">Phenotyping</rdfs:label>
        <rdfs:label xml:lang="de">Phänotypisierung</rdfs:label>
        <skos:definition xml:lang="de">Die Phänotypisierung ist ein Prozess der Identifizierung von Personen mit bestimmten Phänotypen.</skos:definition>
        <skos:definition xml:lang="en">Phenotyping is a process of identifying individuals with certain phenotypes.</skos:definition>
    </owl:Class>
    


    <!-- https://w3id.org/cop/PhenotypingSoftware -->


    <owl:Class rdf:about="https://w3id.org/cop/PhenotypingSoftware">
        <rdfs:subClassOf rdf:resource="https://w3id.org/cop/Software"/>
        <rdfs:subClassOf>
            <owl:Restriction>
                <owl:onProperty rdf:resource="https://w3id.org/cop/implements"/>
                <owl:someValuesFrom rdf:resource="https://w3id.org/cop/PhenotypeAlgorithm"/>
            </owl:Restriction>
        </rdfs:subClassOf>
        <rdfs:subClassOf>
            <owl:Restriction>
                <owl:onProperty rdf:resource="https://w3id.org/cop/realises"/>
                <owl:someValuesFrom rdf:resource="https://w3id.org/cop/Phenotyping"/>
            </owl:Restriction>
        </rdfs:subClassOf>
        <rdfs:comment xml:lang="en">A run of a phenotyping software (implemented phenotype algorithm) realises a phenotyping process.</rdfs:comment>
        <rdfs:comment xml:lang="de">Ein Durchlauf einer Phänotypisierungssoftware (implementierter Phänotypisierungsalgorithmus) realisiert einen Phänotypisierungsprozess.</rdfs:comment>
        <rdfs:label xml:lang="en">Phenotyping software</rdfs:label>
        <rdfs:label xml:lang="de">Phänotypisierungssoftware</rdfs:label>
        <skos:definition xml:lang="en">Phenotyping software is a software implementing a phenotype algorithm.</skos:definition>
        <skos:definition xml:lang="de">Phänotypisierungssoftware ist eine Software, die einen Phänotypisierungsalgorithmus implementiert.</skos:definition>
    </owl:Class>
    


    <!-- https://w3id.org/cop/RestrictedPhenotypeClass -->


    <owl:Class rdf:about="https://w3id.org/cop/RestrictedPhenotypeClass">
        <rdfs:subClassOf rdf:resource="https://w3id.org/cop/PhenotypeClass"/>
        <rdfs:subClassOf>
            <owl:Restriction>
                <owl:onProperty rdf:resource="https://w3id.org/cop/restrictionOf"/>
                <owl:qualifiedCardinality rdf:datatype="http://www.w3.org/2001/XMLSchema#nonNegativeInteger">1</owl:qualifiedCardinality>
                <owl:onClass rdf:resource="https://w3id.org/cop/UnrestrictedPhenotypeClass"/>
            </owl:Restriction>
        </rdfs:subClassOf>
        <rdfs:label xml:lang="de">Eingeschränkte Phänotypklasse</rdfs:label>
        <rdfs:label xml:lang="en">Restricted phenotype class</rdfs:label>
        <skos:altLabel xml:lang="en">Phenotype restriction</skos:altLabel>
        <skos:altLabel xml:lang="de">Phänotyprestriktion</skos:altLabel>
        <skos:definition xml:lang="en">A phenotype class whose extension (the set of instances, i.e., phenotypes) is restricted to a certain value range is called restricted phenotype class.</skos:definition>
        <skos:definition xml:lang="de">Eine Phänotypklasse, deren Erweiterung (die Menge der Instanzen, d.h. der Phänotypen) auf einen bestimmten Wertebereich beschränkt ist, wird als eingeschränkte Phänotypklasse bezeichnet.</skos:definition>
        <skos:example xml:lang="en">Overweight (e.g., BMI over 30)</skos:example>
        <skos:example xml:lang="en">Weight over 100 kg</skos:example>
    </owl:Class>
    


    <!-- https://w3id.org/cop/Software -->


    <owl:Class rdf:about="https://w3id.org/cop/Software">
        <rdfs:subClassOf rdf:resource="https://w3id.org/gfo-light/InformationObject"/>
        <rdfs:subClassOf>
            <owl:Restriction>
                <owl:onProperty rdf:resource="https://w3id.org/cop/implements"/>
                <owl:someValuesFrom rdf:resource="https://w3id.org/cop/Algorithm"/>
            </owl:Restriction>
        </rdfs:subClassOf>
        <rdfs:subClassOf>
            <owl:Restriction>
                <owl:onProperty rdf:resource="https://w3id.org/cop/realises"/>
                <owl:someValuesFrom rdf:resource="https://w3id.org/gfo-light/Process"/>
            </owl:Restriction>
        </rdfs:subClassOf>
        <rdfs:label xml:lang="de">Software</rdfs:label>
        <rdfs:label xml:lang="en">Software</rdfs:label>
        <skos:definition xml:lang="en">Software refers to executable computer programmes including all their components.</skos:definition>
        <skos:definition xml:lang="de">Unter Software versteht man ausführbare Computerprogramme einschließlich aller ihrer Komponenten.</skos:definition>
    </owl:Class>
    


    <!-- https://w3id.org/cop/StaticPhenotypeAlgorithm -->


    <owl:Class rdf:about="https://w3id.org/cop/StaticPhenotypeAlgorithm">
        <rdfs:subClassOf rdf:resource="https://w3id.org/cop/PhenotypeAlgorithm"/>
        <rdfs:subClassOf>
            <owl:Restriction>
                <owl:onProperty rdf:resource="https://w3id.org/cop/applicableFor"/>
                <owl:qualifiedCardinality rdf:datatype="http://www.w3.org/2001/XMLSchema#nonNegativeInteger">1</owl:qualifiedCardinality>
                <owl:onClass rdf:resource="https://w3id.org/cop/PhenotypeQuery"/>
            </owl:Restriction>
        </rdfs:subClassOf>
        <rdfs:label xml:lang="en">Static phenotype algorithm</rdfs:label>
        <rdfs:label xml:lang="de">Statischer Phänotypalgorithmus</rdfs:label>
        <skos:definition xml:lang="en">A static phenotype algorithm is a phenotype algorithm for executing exactly one specific phenotype query.</skos:definition>
        <skos:definition xml:lang="de">Ein statischer Phänotypalgorithmus ist ein Phänotypalgorithmus zur Ausführung genau einer bestimmten Phänotypabfrage.</skos:definition>
    </owl:Class>
    


    <!-- https://w3id.org/cop/StringSpec -->


    <owl:Class rdf:about="https://w3id.org/cop/StringSpec">
        <rdfs:subClassOf rdf:resource="https://w3id.org/cop/DataTypeSpec"/>
        <rdfs:label xml:lang="en">String data type specification</rdfs:label>
    </owl:Class>
    


    <!-- https://w3id.org/cop/Synonym -->


    <owl:Class rdf:about="https://w3id.org/cop/Synonym">
        <rdfs:subClassOf rdf:resource="https://w3id.org/cop/AttributeSpec"/>
        <rdfs:label xml:lang="de">Synonym</rdfs:label>
        <rdfs:label xml:lang="en">Synonym</rdfs:label>
        <skos:definition xml:lang="en">A synonym is a string that has a similar meaning to the title.</skos:definition>
        <skos:definition xml:lang="de">Ein Synonym ist eine Zeichenkette, die eine ähnliche Bedeutung wie der Titel hat.</skos:definition>
    </owl:Class>
    


    <!-- https://w3id.org/cop/TerminologyCode -->


    <owl:Class rdf:about="https://w3id.org/cop/TerminologyCode">
        <rdfs:subClassOf rdf:resource="https://w3id.org/cop/AttributeSpec"/>
        <rdfs:label xml:lang="de">Terminologiecode</rdfs:label>
        <rdfs:label xml:lang="en">Terminology code</rdfs:label>
        <skos:definition xml:lang="en">A terminology code is a code of a terminology (code system).</skos:definition>
        <skos:definition xml:lang="de">Ein Terminologiecode ist ein Code aus einer Terminologie (Codesystem).</skos:definition>
    </owl:Class>
    


    <!-- https://w3id.org/cop/Title -->


    <owl:Class rdf:about="https://w3id.org/cop/Title">
        <rdfs:subClassOf rdf:resource="https://w3id.org/cop/AttributeSpec"/>
        <rdfs:label xml:lang="de">Titel</rdfs:label>
        <rdfs:label xml:lang="en">Title</rdfs:label>
        <skos:definition xml:lang="en">A title is a string designating an entity.</skos:definition>
        <skos:definition xml:lang="de">Ein Titel ist eine Zeichenkette, die eine Entität bezeichnet.</skos:definition>
    </owl:Class>
    


    <!-- https://w3id.org/cop/UnitOfMeasureSpec -->


    <owl:Class rdf:about="https://w3id.org/cop/UnitOfMeasureSpec">
        <rdfs:subClassOf rdf:resource="https://w3id.org/cop/AttributeSpec"/>
        <rdfs:label xml:lang="de">Maßeinheitsspezifikation</rdfs:label>
        <rdfs:label xml:lang="en">Unit of measure specification</rdfs:label>
        <skos:definition xml:lang="en">A unit of measure specification is a specification of a unit of measure.</skos:definition>
        <skos:definition xml:lang="de">Eine Maßeinheitsspezifikation ist eine Spezifikation einer Maßeinheit.</skos:definition>
    </owl:Class>
    


    <!-- https://w3id.org/cop/UnrestrictedPhenotypeClass -->


    <owl:Class rdf:about="https://w3id.org/cop/UnrestrictedPhenotypeClass">
        <rdfs:subClassOf rdf:resource="https://w3id.org/cop/PhenotypeClass"/>
        <rdfs:label xml:lang="de">Uneingeschränkte Phänotypklasse</rdfs:label>
        <rdfs:label xml:lang="en">Unrestricted phenotype class</rdfs:label>
        <skos:definition xml:lang="en">A phenotype class whose extension (the set of instances, i.e., phenotypes) is not restricted to a certain value range is called unrestricted phenotype class.</skos:definition>
        <skos:definition xml:lang="de">Eine Phänotypklasse, deren Erweiterung (die Menge der Instanzen, d.h. der Phänotypen) nicht auf einen bestimmten Wertebereich beschränkt ist, wird als uneingeschränkte Phänotypklasse bezeichnet.</skos:definition>
        <skos:example xml:lang="en">Body Mass Index (BMI)</skos:example>
        <skos:example xml:lang="en">Weight</skos:example>
    </owl:Class>
    


    <!-- https://w3id.org/cop/ValueRangeSpec -->


    <owl:Class rdf:about="https://w3id.org/cop/ValueRangeSpec">
        <rdfs:subClassOf rdf:resource="https://w3id.org/cop/AttributeSpec"/>
        <rdfs:subClassOf>
            <owl:Restriction>
                <owl:onProperty rdf:resource="https://w3id.org/gfo-light/partOf"/>
                <owl:someValuesFrom>
                    <owl:Class>
                        <owl:unionOf rdf:parseType="Collection">
                            <rdf:Description rdf:about="https://w3id.org/cop/BasicRestrictedPhenotypeClassView"/>
                            <rdf:Description rdf:about="https://w3id.org/cop/DerivedRestrictedPhenotypeClassView"/>
                        </owl:unionOf>
                    </owl:Class>
                </owl:someValuesFrom>
            </owl:Restriction>
        </rdfs:subClassOf>
        <rdfs:label xml:lang="en">Value range specification</rdfs:label>
        <rdfs:label xml:lang="de">Wertebereichsspezifikation</rdfs:label>
        <skos:definition xml:lang="en">A value range specification is a specification of the permitted values of an entity (e.g., of a phenotype), either by listing them (e.g., for string values) or by defining the minimum and maximum (e.g., for numerical values).</skos:definition>
        <skos:definition xml:lang="de">Eine Wertebereichsspezifikation ist eine Spezifikation der zulässigen Werte einer Entität (z.B. eines Phänotyps), entweder durch Auflistung (z.B. bei Zeichenkettenwerten) oder durch Definition von Minimum und Maximum (z.B. bei numerischen Werten).</skos:definition>
    </owl:Class>
    


    <!-- https://w3id.org/gfo-light/Attributive -->


    <owl:Class rdf:about="https://w3id.org/gfo-light/Attributive">
        <rdfs:subClassOf rdf:resource="https://w3id.org/gfo-light/ConcreteIndividual"/>
        <rdfs:subClassOf>
            <owl:Restriction>
                <owl:onProperty rdf:resource="https://w3id.org/gfo-light/attributiveOf"/>
                <owl:someValuesFrom rdf:resource="https://w3id.org/gfo-light/Individual"/>
            </owl:Restriction>
        </rdfs:subClassOf>
        <rdfs:comment xml:lang="en">Qualities (attributes, traits, characteristics, etc.) of concrete individuals, relations (relators) between them and roles that objects can play in different contexts are subsumed under the category Attributive.</rdfs:comment>
        <rdfs:label xml:lang="en">Attributive</rdfs:label>
        <skos:definition xml:lang="en">Attributives are individuals that depend on other individuals by some kind of dependency relation.</skos:definition>
    </owl:Class>
    


    <!-- https://w3id.org/gfo-light/Category -->


    <owl:Class rdf:about="https://w3id.org/gfo-light/Category">
        <rdfs:subClassOf rdf:resource="https://w3id.org/gfo-light/Entity"/>
        <rdfs:subClassOf>
            <owl:Restriction>
                <owl:onProperty rdf:resource="https://w3id.org/gfo-light/instantiatedBy"/>
                <owl:allValuesFrom>
                    <owl:Class>
                        <owl:unionOf rdf:parseType="Collection">
                            <rdf:Description rdf:about="https://w3id.org/gfo-light/Category"/>
                            <rdf:Description rdf:about="https://w3id.org/gfo-light/Individual"/>
                        </owl:unionOf>
                    </owl:Class>
                </owl:allValuesFrom>
            </owl:Restriction>
        </rdfs:subClassOf>
        <rdfs:label xml:lang="en">Category</rdfs:label>
        <skos:altLabel xml:lang="en">Class</skos:altLabel>
        <skos:altLabel xml:lang="en">Kind</skos:altLabel>
        <skos:altLabel xml:lang="en">Type</skos:altLabel>
        <skos:definition xml:lang="en">The notion of category covers all abstract entities that can be instantiated by or are predicated of other entities.</skos:definition>
    </owl:Class>
    


    <!-- https://w3id.org/gfo-light/Chronoid -->


    <owl:Class rdf:about="https://w3id.org/gfo-light/Chronoid">
        <rdfs:subClassOf rdf:resource="https://w3id.org/gfo-light/TimeEntity"/>
        <rdfs:subClassOf>
            <owl:Class>
                <owl:unionOf rdf:parseType="Collection">
                    <owl:Class>
                        <owl:intersectionOf rdf:parseType="Collection">
                            <owl:Restriction>
                                <owl:onProperty rdf:resource="https://w3id.org/gfo-light/temporallyFinishedBy"/>
                                <owl:qualifiedCardinality rdf:datatype="http://www.w3.org/2001/XMLSchema#nonNegativeInteger">1</owl:qualifiedCardinality>
                                <owl:onClass rdf:resource="https://w3id.org/gfo-light/TimeBoundary"/>
                            </owl:Restriction>
                            <owl:Restriction>
                                <owl:onProperty rdf:resource="https://w3id.org/gfo-light/temporallyStartedBy"/>
                                <owl:qualifiedCardinality rdf:datatype="http://www.w3.org/2001/XMLSchema#nonNegativeInteger">1</owl:qualifiedCardinality>
                                <owl:onClass rdf:resource="https://w3id.org/gfo-light/TimeBoundary"/>
                            </owl:Restriction>
                        </owl:intersectionOf>
                    </owl:Class>
                    <owl:Class>
                        <owl:intersectionOf rdf:parseType="Collection">
                            <owl:Restriction>
                                <owl:onProperty rdf:resource="https://w3id.org/gfo-light/finishedByDateTimeValue"/>
                                <owl:qualifiedCardinality rdf:datatype="http://www.w3.org/2001/XMLSchema#nonNegativeInteger">1</owl:qualifiedCardinality>
                                <owl:onDataRange rdf:resource="http://www.w3.org/2001/XMLSchema#dateTime"/>
                            </owl:Restriction>
                            <owl:Restriction>
                                <owl:onProperty rdf:resource="https://w3id.org/gfo-light/startedByDateTimeValue"/>
                                <owl:qualifiedCardinality rdf:datatype="http://www.w3.org/2001/XMLSchema#nonNegativeInteger">1</owl:qualifiedCardinality>
                                <owl:onDataRange rdf:resource="http://www.w3.org/2001/XMLSchema#dateTime"/>
                            </owl:Restriction>
                        </owl:intersectionOf>
                    </owl:Class>
                </owl:unionOf>
            </owl:Class>
        </rdfs:subClassOf>
        <rdfs:label xml:lang="en">Chronoid</rdfs:label>
        <skos:altLabel xml:lang="en">Time interval</skos:altLabel>
        <skos:altLabel xml:lang="en">Time period</skos:altLabel>
        <skos:definition xml:lang="en">Chronoids are real-valued time intervals with endpoints.</skos:definition>
        <skos:example xml:lang="en">The time (extension) of a football match (from the start point in time to the end point in time)</skos:example>
    </owl:Class>
    


    <!-- https://w3id.org/gfo-light/ConcreteIndividual -->


    <owl:Class rdf:about="https://w3id.org/gfo-light/ConcreteIndividual">
        <rdfs:subClassOf rdf:resource="https://w3id.org/gfo-light/Individual"/>
        <rdfs:subClassOf>
            <owl:Class>
                <owl:unionOf rdf:parseType="Collection">
                    <owl:Class>
                        <owl:intersectionOf rdf:parseType="Collection">
                            <owl:Restriction>
                                <owl:onProperty rdf:resource="https://w3id.org/gfo-light/finishedByDateTimeValue"/>
                                <owl:qualifiedCardinality rdf:datatype="http://www.w3.org/2001/XMLSchema#nonNegativeInteger">1</owl:qualifiedCardinality>
                                <owl:onDataRange rdf:resource="http://www.w3.org/2001/XMLSchema#dateTime"/>
                            </owl:Restriction>
                            <owl:Restriction>
                                <owl:onProperty rdf:resource="https://w3id.org/gfo-light/startedByDateTimeValue"/>
                                <owl:qualifiedCardinality rdf:datatype="http://www.w3.org/2001/XMLSchema#nonNegativeInteger">1</owl:qualifiedCardinality>
                                <owl:onDataRange rdf:resource="http://www.w3.org/2001/XMLSchema#dateTime"/>
                            </owl:Restriction>
                        </owl:intersectionOf>
                    </owl:Class>
                    <owl:Restriction>
                        <owl:onProperty rdf:resource="https://w3id.org/gfo-light/hasTime"/>
                        <owl:qualifiedCardinality rdf:datatype="http://www.w3.org/2001/XMLSchema#nonNegativeInteger">1</owl:qualifiedCardinality>
                        <owl:onClass rdf:resource="https://w3id.org/gfo-light/TimeEntity"/>
                    </owl:Restriction>
                    <owl:Restriction>
                        <owl:onProperty rdf:resource="https://w3id.org/gfo-light/dateTimeValue"/>
                        <owl:qualifiedCardinality rdf:datatype="http://www.w3.org/2001/XMLSchema#nonNegativeInteger">1</owl:qualifiedCardinality>
                        <owl:onDataRange rdf:resource="http://www.w3.org/2001/XMLSchema#dateTime"/>
                    </owl:Restriction>
                </owl:unionOf>
            </owl:Class>
        </rdfs:subClassOf>
        <rdfs:label xml:lang="en">Concrete individual</rdfs:label>
        <skos:definition xml:lang="en">Concrete individuals are entities that have an immediate relation to time or to space-time. They exist in time.</skos:definition>
    </owl:Class>
    


    <!-- https://w3id.org/gfo-light/Continuant -->


    <owl:Class rdf:about="https://w3id.org/gfo-light/Continuant">
        <rdfs:subClassOf rdf:resource="https://w3id.org/gfo-light/ConcreteIndividual"/>
        <rdfs:subClassOf>
            <owl:Class>
                <owl:unionOf rdf:parseType="Collection">
                    <owl:Class>
                        <owl:intersectionOf rdf:parseType="Collection">
                            <owl:Restriction>
                                <owl:onProperty rdf:resource="https://w3id.org/gfo-light/finishedByDateTimeValue"/>
                                <owl:qualifiedCardinality rdf:datatype="http://www.w3.org/2001/XMLSchema#nonNegativeInteger">1</owl:qualifiedCardinality>
                                <owl:onDataRange rdf:resource="http://www.w3.org/2001/XMLSchema#dateTime"/>
                            </owl:Restriction>
                            <owl:Restriction>
                                <owl:onProperty rdf:resource="https://w3id.org/gfo-light/startedByDateTimeValue"/>
                                <owl:qualifiedCardinality rdf:datatype="http://www.w3.org/2001/XMLSchema#nonNegativeInteger">1</owl:qualifiedCardinality>
                                <owl:onDataRange rdf:resource="http://www.w3.org/2001/XMLSchema#dateTime"/>
                            </owl:Restriction>
                        </owl:intersectionOf>
                    </owl:Class>
                    <owl:Restriction>
                        <owl:onProperty rdf:resource="https://w3id.org/gfo-light/hasTime"/>
                        <owl:qualifiedCardinality rdf:datatype="http://www.w3.org/2001/XMLSchema#nonNegativeInteger">1</owl:qualifiedCardinality>
                        <owl:onClass rdf:resource="https://w3id.org/gfo-light/Chronoid"/>
                    </owl:Restriction>
                </owl:unionOf>
            </owl:Class>
        </rdfs:subClassOf>
        <rdfs:comment xml:lang="en">Social or material (three-dimensional) objects, their groups/aggregates, parts and boundaries (two-, one- and zero-dimensional entities, i.e., surfaces, lines and points) are subsumed under the category Continuant.</rdfs:comment>
        <rdfs:comment xml:lang="en">While the object parts are firmly connected to the entire object, the aggregate members are loose objects. When modelling a person, for example, you could consider their skeleton as an object and as part of the human body. However, if we look at bone finds in the context of anthropology, the skeleton can be modelled as an aggregate of individual bones. Another example is a computer. A kit of computer components is an object aggregate before assembly and an object (a computer) afterwards. However, if the components are thrown into the case without being correctly connected, it is not a computer, but the components are simply located in the case.</rdfs:comment>
        <rdfs:label xml:lang="en">Continuant</rdfs:label>
        <skos:definition xml:lang="en">Continuants are concrete individuals that persist through time and are wholly present at every point of their existence time (lifetime).</skos:definition>
    </owl:Class>
    


    <!-- https://w3id.org/gfo-light/Entity -->


    <owl:Class rdf:about="https://w3id.org/gfo-light/Entity">
        <rdfs:label xml:lang="en">Entity</rdfs:label>
        <skos:definition xml:lang="en">Everything that exists is called an entity.</skos:definition>
    </owl:Class>
    


    <!-- https://w3id.org/gfo-light/Individual -->


    <owl:Class rdf:about="https://w3id.org/gfo-light/Individual">
        <rdfs:subClassOf rdf:resource="https://w3id.org/gfo-light/Entity"/>
        <rdfs:subClassOf>
            <owl:Restriction>
                <owl:onProperty rdf:resource="https://w3id.org/gfo-light/instanceOf"/>
                <owl:someValuesFrom rdf:resource="https://w3id.org/gfo-light/Category"/>
            </owl:Restriction>
        </rdfs:subClassOf>
        <rdfs:label xml:lang="en">Individual</rdfs:label>
        <skos:definition xml:lang="en">Individuals are entities which cannot be further instantiated.</skos:definition>
    </owl:Class>
    


    <!-- https://w3id.org/gfo-light/InformationObject -->


    <owl:Class rdf:about="https://w3id.org/gfo-light/InformationObject">
        <rdfs:subClassOf rdf:resource="https://w3id.org/gfo-light/Object"/>
        <rdfs:subClassOf>
            <owl:Restriction>
                <owl:onProperty rdf:resource="https://w3id.org/gfo-light/represents"/>
                <owl:someValuesFrom rdf:resource="https://w3id.org/gfo-light/Entity"/>
            </owl:Restriction>
        </rdfs:subClassOf>
        <rdfs:label xml:lang="en">Information object</rdfs:label>
        <skos:definition xml:lang="en">Information objects are symbolic entities that denote/designate, describe, specify or represent other entities.</skos:definition>
        <skos:example xml:lang="en">Computer programme</skos:example>
        <skos:example xml:lang="en">Description</skos:example>
        <skos:example xml:lang="en">Diagram</skos:example>
        <skos:example xml:lang="en">Model</skos:example>
        <skos:example xml:lang="en">Title</skos:example>
    </owl:Class>
    


    <!-- https://w3id.org/gfo-light/Line -->


    <owl:Class rdf:about="https://w3id.org/gfo-light/Line">
        <rdfs:subClassOf rdf:resource="https://w3id.org/gfo-light/ObjectBoundary"/>
        <rdfs:subClassOf>
            <owl:Restriction>
                <owl:onProperty rdf:resource="https://w3id.org/gfo-light/boundaryOf"/>
                <owl:allValuesFrom rdf:resource="https://w3id.org/gfo-light/Surface"/>
            </owl:Restriction>
        </rdfs:subClassOf>
        <rdfs:comment xml:lang="en">Lines are not necessarily straight. They can be, for example, curves or broken lines that pass through various points and form a corner, a triangle or a polygon.</rdfs:comment>
        <rdfs:label xml:lang="en">Line</rdfs:label>
        <skos:definition xml:lang="en">A line is a 1-dimensional object boundary.</skos:definition>
        <skos:example xml:lang="en">Boundary line of the football field</skos:example>
        <skos:example xml:lang="en">Longitudinal axis of the human skeleton</skos:example>
    </owl:Class>
    


    <!-- https://w3id.org/gfo-light/Object -->


    <owl:Class rdf:about="https://w3id.org/gfo-light/Object">
        <rdfs:subClassOf rdf:resource="https://w3id.org/gfo-light/Continuant"/>
        <rdfs:label xml:lang="en">Object</rdfs:label>
        <skos:definition xml:lang="en">Objects are social or material entities that can exist independently of each other.</skos:definition>
        <skos:example xml:lang="en">Bone</skos:example>
        <skos:example xml:lang="en">Chopstick</skos:example>
        <skos:example xml:lang="en">Computer</skos:example>
        <skos:example xml:lang="en">Person</skos:example>
    </owl:Class>
    


    <!-- https://w3id.org/gfo-light/ObjectAggregate -->


    <owl:Class rdf:about="https://w3id.org/gfo-light/ObjectAggregate">
        <rdfs:subClassOf rdf:resource="https://w3id.org/gfo-light/Continuant"/>
        <rdfs:subClassOf>
            <owl:Restriction>
                <owl:onProperty rdf:resource="https://w3id.org/gfo-light/hasMember"/>
                <owl:someValuesFrom>
                    <owl:Class>
                        <owl:unionOf rdf:parseType="Collection">
                            <rdf:Description rdf:about="https://w3id.org/gfo-light/Object"/>
                            <rdf:Description rdf:about="https://w3id.org/gfo-light/ObjectAggregate"/>
                        </owl:unionOf>
                    </owl:Class>
                </owl:someValuesFrom>
            </owl:Restriction>
        </rdfs:subClassOf>
        <rdfs:label xml:lang="en">Object aggregate</rdfs:label>
        <skos:altLabel xml:lang="en">Collection</skos:altLabel>
        <skos:altLabel xml:lang="en">Collective</skos:altLabel>
        <skos:altLabel xml:lang="en">Group</skos:altLabel>
        <skos:definition xml:lang="en">Object aggregates are groups of objects that together form a unit.</skos:definition>
        <skos:example xml:lang="en">Research group</skos:example>
        <skos:example xml:lang="en">Sports team</skos:example>
    </owl:Class>
    


    <!-- https://w3id.org/gfo-light/ObjectBoundary -->


    <owl:Class rdf:about="https://w3id.org/gfo-light/ObjectBoundary">
        <rdfs:subClassOf rdf:resource="https://w3id.org/gfo-light/Continuant"/>
        <rdfs:subClassOf>
            <owl:Restriction>
                <owl:onProperty rdf:resource="https://w3id.org/gfo-light/hasOwner"/>
                <owl:someValuesFrom rdf:resource="https://w3id.org/gfo-light/Object"/>
            </owl:Restriction>
        </rdfs:subClassOf>
        <rdfs:label xml:lang="en">Object boundary</rdfs:label>
        <skos:definition xml:lang="en">Object boundaries are 0-, 1-, or 2-dimensional (visible or imaginary) entities (i.e., points, lines and surfaces) that border objects (natural boundaries) or are located inside them (inner boundaries).</skos:definition>
    </owl:Class>
    


    <!-- https://w3id.org/gfo-light/ObjectPart -->


    <owl:Class rdf:about="https://w3id.org/gfo-light/ObjectPart">
        <rdfs:subClassOf rdf:resource="https://w3id.org/gfo-light/Continuant"/>
        <rdfs:subClassOf>
            <owl:Restriction>
                <owl:onProperty rdf:resource="https://w3id.org/gfo-light/partOf"/>
                <owl:someValuesFrom rdf:resource="https://w3id.org/gfo-light/Object"/>
            </owl:Restriction>
        </rdfs:subClassOf>
        <rdfs:label xml:lang="en">Object part</rdfs:label>
        <skos:definition xml:lang="en">Object parts are material entities that cannot exist independently of the corresponding whole object.</skos:definition>
        <skos:example xml:lang="en">Part of a bone</skos:example>
        <skos:example xml:lang="en">Part of a chopstick</skos:example>
    </owl:Class>
    


    <!-- https://w3id.org/gfo-light/Point -->


    <owl:Class rdf:about="https://w3id.org/gfo-light/Point">
        <rdfs:subClassOf rdf:resource="https://w3id.org/gfo-light/ObjectBoundary"/>
        <rdfs:subClassOf>
            <owl:Restriction>
                <owl:onProperty rdf:resource="https://w3id.org/gfo-light/boundaryOf"/>
                <owl:allValuesFrom rdf:resource="https://w3id.org/gfo-light/Line"/>
            </owl:Restriction>
        </rdfs:subClassOf>
        <rdfs:label xml:lang="en">Point</rdfs:label>
        <skos:definition xml:lang="en">A point is a 0-dimensional object boundary.</skos:definition>
        <skos:example xml:lang="en">Gonion</skos:example>
        <skos:example xml:lang="en">Penalty spot</skos:example>
    </owl:Class>
    


    <!-- https://w3id.org/gfo-light/Process -->


    <owl:Class rdf:about="https://w3id.org/gfo-light/Process">
        <rdfs:subClassOf rdf:resource="https://w3id.org/gfo-light/ProcessualEntity"/>
        <rdfs:subClassOf>
            <owl:Restriction>
                <owl:onProperty rdf:resource="https://w3id.org/gfo-light/hasProcessPart"/>
                <owl:someValuesFrom>
                    <owl:Class>
                        <owl:unionOf rdf:parseType="Collection">
                            <rdf:Description rdf:about="https://w3id.org/gfo-light/Attributive"/>
                            <rdf:Description rdf:about="https://w3id.org/gfo-light/Process"/>
                            <rdf:Description rdf:about="https://w3id.org/gfo-light/Situation"/>
                        </owl:unionOf>
                    </owl:Class>
                </owl:someValuesFrom>
            </owl:Restriction>
        </rdfs:subClassOf>
        <rdfs:comment xml:lang="en">Processes represent dynamic knowledge.</rdfs:comment>
        <rdfs:label xml:lang="en">Process</rdfs:label>
        <skos:definition xml:lang="en">Processes are concrete individuals that happen in time and have a temporal extension (a chronoid).</skos:definition>
        <skos:example xml:lang="en">A treatment of a patient in a hospital</skos:example>
        <skos:example xml:lang="en">Football match</skos:example>
        <skos:example xml:lang="en">The course of an illness</skos:example>
        <skos:example xml:lang="en">The first half of the match</skos:example>
    </owl:Class>
    


    <!-- https://w3id.org/gfo-light/ProcessAggregate -->


    <owl:Class rdf:about="https://w3id.org/gfo-light/ProcessAggregate">
        <rdfs:subClassOf rdf:resource="https://w3id.org/gfo-light/ProcessualEntity"/>
        <rdfs:subClassOf>
            <owl:Restriction>
                <owl:onProperty rdf:resource="https://w3id.org/gfo-light/hasMember"/>
                <owl:someValuesFrom rdf:resource="https://w3id.org/gfo-light/ProcessualEntity"/>
            </owl:Restriction>
        </rdfs:subClassOf>
        <rdfs:label xml:lang="en">Process aggregate</rdfs:label>
        <skos:definition xml:lang="en">Process aggregates are sets of processes that are contextually related but not temporally connected.</skos:definition>
        <skos:example xml:lang="en">All football matches in a league season</skos:example>
        <skos:example xml:lang="en">Series of lectures in a semester</skos:example>
    </owl:Class>
    


    <!-- https://w3id.org/gfo-light/ProcessualEntity -->


    <owl:Class rdf:about="https://w3id.org/gfo-light/ProcessualEntity">
        <rdfs:subClassOf rdf:resource="https://w3id.org/gfo-light/ConcreteIndividual"/>
        <rdfs:subClassOf>
            <owl:Class>
                <owl:unionOf rdf:parseType="Collection">
                    <owl:Class>
                        <owl:intersectionOf rdf:parseType="Collection">
                            <owl:Restriction>
                                <owl:onProperty rdf:resource="https://w3id.org/gfo-light/finishedByDateTimeValue"/>
                                <owl:qualifiedCardinality rdf:datatype="http://www.w3.org/2001/XMLSchema#nonNegativeInteger">1</owl:qualifiedCardinality>
                                <owl:onDataRange rdf:resource="http://www.w3.org/2001/XMLSchema#dateTime"/>
                            </owl:Restriction>
                            <owl:Restriction>
                                <owl:onProperty rdf:resource="https://w3id.org/gfo-light/startedByDateTimeValue"/>
                                <owl:qualifiedCardinality rdf:datatype="http://www.w3.org/2001/XMLSchema#nonNegativeInteger">1</owl:qualifiedCardinality>
                                <owl:onDataRange rdf:resource="http://www.w3.org/2001/XMLSchema#dateTime"/>
                            </owl:Restriction>
                        </owl:intersectionOf>
                    </owl:Class>
                    <owl:Restriction>
                        <owl:onProperty rdf:resource="https://w3id.org/gfo-light/hasTime"/>
                        <owl:qualifiedCardinality rdf:datatype="http://www.w3.org/2001/XMLSchema#nonNegativeInteger">1</owl:qualifiedCardinality>
                        <owl:onClass rdf:resource="https://w3id.org/gfo-light/Chronoid"/>
                    </owl:Restriction>
                </owl:unionOf>
            </owl:Class>
        </rdfs:subClassOf>
        <rdfs:subClassOf>
            <owl:Restriction>
                <owl:onProperty rdf:resource="https://w3id.org/gfo-light/hasParticipant"/>
                <owl:allValuesFrom rdf:resource="https://w3id.org/gfo-light/Continuant"/>
            </owl:Restriction>
        </rdfs:subClassOf>
        <rdfs:label xml:lang="en">Processual entity</rdfs:label>
        <skos:definition xml:lang="en">Processual entities include processes and processual aggregates.</skos:definition>
    </owl:Class>
    


    <!-- https://w3id.org/gfo-light/Quality -->


    <owl:Class rdf:about="https://w3id.org/gfo-light/Quality">
        <rdfs:subClassOf rdf:resource="https://w3id.org/gfo-light/Attributive"/>
        <rdfs:subClassOf>
            <owl:Restriction>
                <owl:onProperty rdf:resource="https://w3id.org/gfo-light/qualityOf"/>
                <owl:qualifiedCardinality rdf:datatype="http://www.w3.org/2001/XMLSchema#nonNegativeInteger">1</owl:qualifiedCardinality>
                <owl:onClass rdf:resource="https://w3id.org/gfo-light/Individual"/>
            </owl:Restriction>
        </rdfs:subClassOf>
        <rdfs:comment xml:lang="en">Qualities can possess values.</rdfs:comment>
        <rdfs:label xml:lang="en">Quality</rdfs:label>
        <skos:altLabel xml:lang="en">Attribute</skos:altLabel>
        <skos:altLabel xml:lang="en">Characteristic</skos:altLabel>
        <skos:altLabel xml:lang="en">Feature</skos:altLabel>
        <skos:altLabel xml:lang="en">Property</skos:altLabel>
        <skos:altLabel xml:lang="en">Trait</skos:altLabel>
        <skos:definition xml:lang="en">Qualities are attributives that typically inhere in its bearer.</skos:definition>
        <skos:example xml:lang="en">Observable or measurable characteristics of single objects, e.g., persons, (such as weight and height, laboratory parameters or symptoms)</skos:example>
        <skos:example xml:lang="en">Qualities of object groups (e.g., goals scored by a football team in a match)</skos:example>
        <skos:example xml:lang="en">Qualities of processes (e.g., the number of spectators as quality of a football match)</skos:example>
    </owl:Class>
    


    <!-- https://w3id.org/gfo-light/Relator -->


    <owl:Class rdf:about="https://w3id.org/gfo-light/Relator">
        <rdfs:subClassOf rdf:resource="https://w3id.org/gfo-light/Attributive"/>
        <rdfs:subClassOf>
            <owl:Restriction>
                <owl:onProperty rdf:resource="https://w3id.org/gfo-light/containsRole"/>
                <owl:someValuesFrom rdf:resource="https://w3id.org/gfo-light/Role"/>
            </owl:Restriction>
        </rdfs:subClassOf>
        <rdfs:subClassOf>
            <owl:Restriction>
                <owl:onProperty rdf:resource="https://w3id.org/gfo-light/relates"/>
                <owl:minQualifiedCardinality rdf:datatype="http://www.w3.org/2001/XMLSchema#nonNegativeInteger">2</owl:minQualifiedCardinality>
                <owl:onClass rdf:resource="https://w3id.org/gfo-light/Continuant"/>
            </owl:Restriction>
        </rdfs:subClassOf>
        <rdfs:comment xml:lang="en">A relator represents an individual relation instance.</rdfs:comment>
        <rdfs:label xml:lang="en">Relator</rdfs:label>
        <skos:definition xml:lang="en">Relators are attributives that connect other entities (role players) by relational roles (played by role players).</skos:definition>
        <skos:example xml:lang="en">A relator describing the relative location of an object (playing the target object role) in relation to another object (playing the reference object role), e.g., the location of a person relative to the city centre or the location of an anatomical structure relative to the longitudinal axis</skos:example>
        <skos:example xml:lang="en">A winner-loser relator connecting a winner and a loser team by a winner and a loser role</skos:example>
        <skos:example xml:lang="en">The marriage (relator) of John and Mary (in which Mary plays the wife role and John the husband role)</skos:example>
    </owl:Class>
    


    <!-- https://w3id.org/gfo-light/Role -->


    <owl:Class rdf:about="https://w3id.org/gfo-light/Role">
        <rdfs:subClassOf rdf:resource="https://w3id.org/gfo-light/Attributive"/>
        <rdfs:subClassOf>
            <owl:Restriction>
                <owl:onProperty rdf:resource="https://w3id.org/gfo-light/playedBy"/>
                <owl:qualifiedCardinality rdf:datatype="http://www.w3.org/2001/XMLSchema#nonNegativeInteger">1</owl:qualifiedCardinality>
                <owl:onClass rdf:resource="https://w3id.org/gfo-light/Continuant"/>
            </owl:Restriction>
        </rdfs:subClassOf>
        <rdfs:subClassOf>
            <owl:Restriction>
                <owl:onProperty rdf:resource="https://w3id.org/gfo-light/roleIn"/>
                <owl:qualifiedCardinality rdf:datatype="http://www.w3.org/2001/XMLSchema#nonNegativeInteger">1</owl:qualifiedCardinality>
                <owl:onClass>
                    <owl:Class>
                        <owl:unionOf rdf:parseType="Collection">
                            <rdf:Description rdf:about="https://w3id.org/gfo-light/Object"/>
                            <rdf:Description rdf:about="https://w3id.org/gfo-light/ObjectAggregate"/>
                            <rdf:Description rdf:about="https://w3id.org/gfo-light/ProcessualEntity"/>
                            <rdf:Description rdf:about="https://w3id.org/gfo-light/Relator"/>
                            <rdf:Description rdf:about="https://w3id.org/gfo-light/SituationalEntity"/>
                        </owl:unionOf>
                    </owl:Class>
                </owl:onClass>
            </owl:Restriction>
        </rdfs:subClassOf>
        <rdfs:comment xml:lang="en">An object part can play a (e.g., functional) role in the whole object (e.g., the processor is part of the computer and has the task/function/role to process commands). A member (object) of a social group (object aggregate) can play a social role in that group (e.g., John is member of the football team and plays the role of midfielder). Objects can play processual or situational roles in processes (e.g., team A plays the home team role and team B plays the visiting team role in a football match) or situations (e.g., scorer and assistant role in a goal situation or roles played by a doctor and a patient in a risk/adverse situation in hospital) in which they participate. Objects can play relational roles in a relation/relator (e.g., wife role and husband role of the marriage relator).</rdfs:comment>
        <rdfs:label xml:lang="en">Role</rdfs:label>
        <skos:definition xml:lang="en">A role is a relational entity that links a continuant (role player) with some context (object, object aggregate, processual entity, situational entity, relator), in which the continuant plays that role.</skos:definition>
        <skos:example xml:lang="en">John is member of the football team and plays the role of midfielder.</skos:example>
        <skos:example xml:lang="en">Roles played by a doctor and a patient in a risk/adverse situation in hospital</skos:example>
        <skos:example xml:lang="en">Target object role and reference object role of a relative location relator (describes the relative location of an object playing the target object role in relation to another object playing the reference object role)</skos:example>
        <skos:example xml:lang="en">Team A plays the home team role and team B plays the visiting team role in a football match.</skos:example>
        <skos:example xml:lang="en">The processor is part of the computer and has the task/function/role to process commands.</skos:example>
        <skos:example xml:lang="en">Wife role and husband role of the marriage relator</skos:example>
        <skos:example xml:lang="en">Winner team role and loser team role of the winner-loser relator</skos:example>
    </owl:Class>
    


    <!-- https://w3id.org/gfo-light/Situation -->


    <owl:Class rdf:about="https://w3id.org/gfo-light/Situation">
        <rdfs:subClassOf rdf:resource="https://w3id.org/gfo-light/SituationalEntity"/>
        <rdfs:subClassOf>
            <owl:Restriction>
                <owl:onProperty rdf:resource="https://w3id.org/gfo-light/hasSituationPart"/>
                <owl:someValuesFrom>
                    <owl:Class>
                        <owl:unionOf rdf:parseType="Collection">
                            <rdf:Description rdf:about="https://w3id.org/gfo-light/Attributive"/>
                            <rdf:Description rdf:about="https://w3id.org/gfo-light/Situation"/>
                        </owl:unionOf>
                    </owl:Class>
                </owl:someValuesFrom>
            </owl:Restriction>
        </rdfs:subClassOf>
        <rdfs:comment xml:lang="en">A situation can exist at a certain point in time or during a certain period of time and can be part or result of a process or another situation.</rdfs:comment>
        <rdfs:comment xml:lang="en">Situations represent static knowledge.</rdfs:comment>
        <rdfs:label xml:lang="en">Situation</rdfs:label>
        <skos:definition xml:lang="en">Situations are combinations/constellations of attributives that belong together in the context of the use case under consideration.</skos:definition>
        <skos:example xml:lang="en">A risk situation when treating a patient in hospital if his laboratory values (qualities) are in the critical range over a certain period of time</skos:example>
        <skos:example xml:lang="en">The situation after the wedding of John and Mary (i.e., the situation in which they are married containing the marriage relator with a husband and a wife role)</skos:example>
        <skos:example xml:lang="en">The situation at the end of a football match containing players&apos; qualities (e.g., number of goals or assists), teams&apos; qualities (e.g., number of goals or ball possession) and a winner-loser relator with one team playing the winner role and the other team playing the loser role</skos:example>
    </owl:Class>
    


    <!-- https://w3id.org/gfo-light/SituationAggregate -->


    <owl:Class rdf:about="https://w3id.org/gfo-light/SituationAggregate">
        <rdfs:subClassOf rdf:resource="https://w3id.org/gfo-light/SituationalEntity"/>
        <rdfs:subClassOf>
            <owl:Restriction>
                <owl:onProperty rdf:resource="https://w3id.org/gfo-light/hasMember"/>
                <owl:someValuesFrom rdf:resource="https://w3id.org/gfo-light/SituationalEntity"/>
            </owl:Restriction>
        </rdfs:subClassOf>
        <rdfs:label xml:lang="en">Situation aggregate</rdfs:label>
        <skos:definition xml:lang="en">Situation aggregates are sets of situations that are contextually related but not temporally connected.</skos:definition>
        <skos:example xml:lang="en">All phases of increased temperature in the course of an illness</skos:example>
    </owl:Class>
    


    <!-- https://w3id.org/gfo-light/SituationalEntity -->


    <owl:Class rdf:about="https://w3id.org/gfo-light/SituationalEntity">
        <rdfs:subClassOf rdf:resource="https://w3id.org/gfo-light/ConcreteIndividual"/>
        <rdfs:subClassOf>
            <owl:Restriction>
                <owl:onProperty rdf:resource="https://w3id.org/gfo-light/hasParticipant"/>
                <owl:allValuesFrom rdf:resource="https://w3id.org/gfo-light/Continuant"/>
            </owl:Restriction>
        </rdfs:subClassOf>
        <rdfs:label xml:lang="en">Situational entity</rdfs:label>
        <skos:definition xml:lang="en">Situational entities include situations and situational aggregates.</skos:definition>
    </owl:Class>
    


    <!-- https://w3id.org/gfo-light/Surface -->


    <owl:Class rdf:about="https://w3id.org/gfo-light/Surface">
        <rdfs:subClassOf rdf:resource="https://w3id.org/gfo-light/ObjectBoundary"/>
        <rdfs:subClassOf>
            <owl:Restriction>
                <owl:onProperty rdf:resource="https://w3id.org/gfo-light/boundaryOf"/>
                <owl:allValuesFrom rdf:resource="https://w3id.org/gfo-light/Object"/>
            </owl:Restriction>
        </rdfs:subClassOf>
        <rdfs:label xml:lang="en">Surface</rdfs:label>
        <skos:definition xml:lang="en">A surface is a 2-dimensional object boundary.</skos:definition>
        <skos:example xml:lang="en">Frontal plane of the human skeleton</skos:example>
        <skos:example xml:lang="en">Surface of the football field</skos:example>
    </owl:Class>
    


    <!-- https://w3id.org/gfo-light/TimeBoundary -->


    <owl:Class rdf:about="https://w3id.org/gfo-light/TimeBoundary">
        <rdfs:subClassOf rdf:resource="https://w3id.org/gfo-light/TimeEntity"/>
        <rdfs:subClassOf>
            <owl:Restriction>
                <owl:onProperty rdf:resource="https://w3id.org/gfo-light/dateTimeValue"/>
                <owl:qualifiedCardinality rdf:datatype="http://www.w3.org/2001/XMLSchema#nonNegativeInteger">1</owl:qualifiedCardinality>
                <owl:onDataRange rdf:resource="http://www.w3.org/2001/XMLSchema#dateTime"/>
            </owl:Restriction>
        </rdfs:subClassOf>
        <rdfs:label xml:lang="en">Time boundary</rdfs:label>
        <skos:altLabel xml:lang="en">Point in time</skos:altLabel>
        <skos:altLabel xml:lang="en">Time point</skos:altLabel>
        <skos:example xml:lang="en">Start point in time of a football match</skos:example>
    </owl:Class>
    


    <!-- https://w3id.org/gfo-light/TimeEntity -->


    <owl:Class rdf:about="https://w3id.org/gfo-light/TimeEntity">
        <rdfs:subClassOf rdf:resource="https://w3id.org/gfo-light/Individual"/>
        <rdfs:comment xml:lang="en">The time entities defined in GFO-light are points in time (time boundaries) and time intervals/periods (chronoids), which consist of points in time.</rdfs:comment>
        <rdfs:label xml:lang="en">Time entity</rdfs:label>
    </owl:Class>
</rdf:RDF>



<!-- Generated by the OWL API (version 5.1.18) https://github.com/owlcs/owlapi/ -->


